@prefix :        <http://www.semanticweb.org/mpuebla/ontologies/2015/8/OntologyOfSpatialObject#> .
@prefix rdfs:    <http://www.w3.org/2000/01/rdf-schema#> .
@prefix ontologyofspatialobject:  <http://www.semanticweb.org/mpuebla/ontologies/2015/8/OntologyOfSpatialObject#> .
@prefix swrl:    <http://www.w3.org/2003/11/swrl#> .
@prefix terms:   <http://purl.org/dc/terms/> .
@prefix owl:     <http://www.w3.org/2002/07/owl#> .
@prefix xsd:     <http://www.w3.org/2001/XMLSchema#> .
@prefix swrlb:   <http://www.w3.org/2003/11/swrlb#> .
@prefix rdf:     <http://www.w3.org/1999/02/22-rdf-syntax-ns#> .

ontologyofspatialobject:meadow
      a       owl:Class ;
      rdfs:comment "meadow.  a small, poorly drained area dominated by grassy vegetation"@en ;
      rdfs:subClassOf ontologyofspatialobject:Vegetation .

ontologyofspatialobject:weir-s-
      a       owl:Class ;
      rdfs:comment "weir(s).  a small dam in a stream, designed to raise the water level or to divert stream flow through a desired channel"@en ;
      rdfs:subClassOf ontologyofspatialobject:Spot .

ontologyofspatialobject:section-of-harbor
      a       owl:Class ;
      rdfs:comment "section of harbor.  "@en ;
      rdfs:subClassOf ontologyofspatialobject:Hydrographic .

ontologyofspatialobject:aerodrome
      a       owl:Class ;
      rdfs:comment "Aerodrome in the United Kingdom or Airport in North America is used to map the main area details (other than helicopters only)"@en ;
      rdfs:subClassOf ontologyofspatialobject:aeroway .

ontologyofspatialobject:farmstead
      a       owl:Class ;
      rdfs:comment "farmstead.  the buildings and adjacent service areas of a farm"@en ;
      rdfs:subClassOf ontologyofspatialobject:Spot .

ontologyofspatialobject:tongue
      a       owl:Class ;
      rdfs:comment "tongue.  an elongate (tongue-like) extension of a flat sea floor into an adjacent higher feature"@en ;
      rdfs:subClassOf ontologyofspatialobject:Undersea .

ontologyofspatialobject:refugee-camp
      a       owl:Class ;
      rdfs:comment "refugee camp.  a camp used by refugees"@en ;
      rdfs:subClassOf ontologyofspatialobject:Spot .

ontologyofspatialobject:intermittent-ponds
      a       owl:Class ;
      rdfs:comment "intermittent ponds.  "@en ;
      rdfs:subClassOf ontologyofspatialobject:Hydrographic .

ontologyofspatialobject:style
      a       owl:FunctionalProperty , owl:DatatypeProperty ;
      rdfs:comment "style"@en ;
      rdfs:domain ontologyofspatialobject:SpatialObject ;
      rdfs:range xsd:string ;
      rdfs:subPropertyOf ontologyofspatialobject:gonameDataProperty .

ontologyofspatialobject:cairn
      a       owl:Class ;
      rdfs:comment "cairn.  a heap of stones erected as a landmark or for other purposes"@en ;
      rdfs:subClassOf ontologyofspatialobject:Spot .

ontologyofspatialobject:desert
      a       owl:Class ;
      rdfs:comment "desert.  a large area with little or no vegetation due to extreme environmental conditions"@en ;
      rdfs:subClassOf ontologyofspatialobject:Hypsographic .

ontologyofspatialobject:equal
      a       owl:TransitiveProperty , owl:ObjectProperty , owl:SymmetricProperty , owl:ReflexiveProperty ;
      rdfs:comment """Two geometries are equal if they occupy the same space.

http://esri.github.io/geometry-api-java/doc/Equals.html"""@en ;
      rdfs:domain ontologyofspatialobject:SpatialObject ;
      rdfs:range ontologyofspatialobject:SpatialObject ;
      rdfs:subPropertyOf ontologyofspatialobject:topological ;
      owl:propertyDisjointWith
              ontologyofspatialobject:touches , ontologyofspatialobject:overlap .

ontologyofspatialobject:oil-pipeline
      a       owl:Class ;
      rdfs:comment "oil pipeline.  a pipeline used for transporting oil"@en ;
      rdfs:subClassOf ontologyofspatialobject:Road .

ontologyofspatialobject:license
      a       owl:AnnotationProperty ;
      rdfs:comment "Por definir"@es .

ontologyofspatialobject:ore-treatment-plant
      a       owl:Class ;
      rdfs:comment "ore treatment plant.  a facility for improving the metal content of ore by concentration"@en ;
      rdfs:subClassOf ontologyofspatialobject:Spot .

ontologyofspatialobject:continentCode
      a       owl:FunctionalProperty , owl:DatatypeProperty ;
      rdfs:comment "continentCode"@en ;
      rdfs:domain ontologyofspatialobject:SpatialObject ;
      rdfs:range xsd:string ;
      rdfs:subPropertyOf ontologyofspatialobject:gonameDataProperty .

ontologyofspatialobject:inside
      a       owl:TransitiveProperty , owl:ObjectProperty , owl:ReflexiveProperty ;
      rdfs:comment """One geometry is within another if it is a subset of the other geometry and their interiors have at least one point in common. Within is the inverse of Contains.


Contenido en. En ocasiones se utiliza el termino \"Within\"

http://esri.github.io/geometry-api-java/doc/Within.html"""@en ;
      rdfs:domain ontologyofspatialobject:SpatialObject ;
      rdfs:range ontologyofspatialobject:SpatialObject ;
      rdfs:subPropertyOf ontologyofspatialobject:topological ;
      owl:inverseOf ontologyofspatialobject:contains .

ontologyofspatialobject:section-of-lake
      a       owl:Class ;
      rdfs:comment "section of lake.  "@en ;
      rdfs:subClassOf ontologyofspatialobject:Hydrographic .

ontologyofspatialobject:palm-tree-reserve
      a       owl:Class ;
      rdfs:comment "palm tree reserve.  an area of palm trees where use is controlled"@en ;
      rdfs:subClassOf ontologyofspatialobject:Area .

<urn:swrl#latitudx>
      a       swrl:Variable .

<urn:swrl#latitud>
      a       swrl:Variable .

ontologyofspatialobject:olive-oil-mill
      a       owl:Class ;
      rdfs:comment "olive oil mill.  a mill where oil is extracted from olives"@en ;
      rdfs:subClassOf ontologyofspatialobject:Spot .

ontologyofspatialobject:religious-site
      a       owl:Class ;
      rdfs:comment "religious site.  an ancient site of significant religious importance"@en ;
      rdfs:subClassOf ontologyofspatialobject:Spot .

ontologyofspatialobject:fishing-area
      a       owl:Class ;
      rdfs:comment "fishing area.  a fishing ground, bank or area where fishermen go to catch fish"@en ;
      rdfs:subClassOf ontologyofspatialobject:Hydrographic .

ontologyofspatialobject:spring-s-
      a       owl:Class ;
      rdfs:comment "spring(s).  a place where ground water flows naturally out of the ground"@en ;
      rdfs:subClassOf ontologyofspatialobject:Hydrographic .

ontologyofspatialobject:novitiate
      a       owl:Class ;
      rdfs:comment "novitiate.  a religious house or school where novices are trained"@en ;
      rdfs:subClassOf ontologyofspatialobject:Spot .

ontologyofspatialobject:mountain
      a       owl:Class ;
      rdfs:comment "mountain.  an elevation standing high above the surrounding area with small summit area, steep slopes and local relief of 300m or more"@en , "mountain.  a well-delineated subdivision of a large and complex positive feature"@en ;
      rdfs:subClassOf ontologyofspatialobject:Hypsographic , ontologyofspatialobject:Undersea .

ontologyofspatialobject:salt-pond
      a       owl:Class ;
      rdfs:comment "salt pond.  a small standing body of salt water often in a marsh or swamp, usually along a seacoast"@en ;
      rdfs:subClassOf ontologyofspatialobject:Hydrographic .

ontologyofspatialobject:moor-s-
      a       owl:Class ;
      rdfs:comment "moor(s).  an area of open ground overlaid with wet peaty soils"@en ;
      rdfs:subClassOf ontologyofspatialobject:Hydrographic .

ontologyofspatialobject:ledge
      a       owl:Class ;
      rdfs:comment "ledge.  a rocky projection or outcrop, commonly linear and near shore"@en ;
      rdfs:subClassOf ontologyofspatialobject:Undersea .

ontologyofspatialobject:mud-flat-s-
      a       owl:Class ;
      rdfs:comment "mud flat(s).  a relatively level area of mud either between high and low tide lines, or subject to flooding"@en ;
      rdfs:subClassOf ontologyofspatialobject:Hydrographic .

ontologyofspatialobject:quicksand
      a       owl:Class ;
      rdfs:comment "quicksand.  an area where loose sand with water moving through it may become unstable when heavy objects are placed at the surface, causing them to sink"@en ;
      rdfs:subClassOf ontologyofspatialobject:Area .

ontologyofspatialobject:bush-es-
      a       owl:Class ;
      rdfs:comment "bush(es).  a small clump of conspicuous bushes in an otherwise bare area"@en ;
      rdfs:subClassOf ontologyofspatialobject:Vegetation .

ontologyofspatialobject:title
      a       owl:DatatypeProperty ;
      rdfs:comment "The article title"@en ;
      rdfs:domain ontologyofspatialobject:SpatialObject ;
      rdfs:range xsd:string ;
      rdfs:subPropertyOf ontologyofspatialobject:wikipediaDataProperty .

ontologyofspatialobject:Hydrographic
      a       owl:Class ;
      rdfs:comment "H stream, lake, ..."@en , "This is used to described different types of waterways. When mapping the way of a river, stream, drain, canal, etc. See the page titled Waterways(\"http://wiki.openstreetmap.org/wiki/Waterways\") for an introduction on its usage."@en ;
      rdfs:subClassOf ontologyofspatialobject:GeonameConcept .

ontologyofspatialobject:section-of-populated-place
      a       owl:Class ;
      rdfs:comment "section of populated place.  "@en ;
      rdfs:subClassOf ontologyofspatialobject:PopulatedPlace .

ontologyofspatialobject:cemetery
      a       owl:Class ;
      rdfs:comment "cemetery.  a burial place or ground"@en ;
      rdfs:subClassOf ontologyofspatialobject:Spot .

ontologyofspatialobject:fossilized-forest
      a       owl:Class ;
      rdfs:comment "fossilized forest.  a forest fossilized by geologic processes and now exposed at the earth's surface"@en ;
      rdfs:subClassOf ontologyofspatialobject:Vegetation .

ontologyofspatialobject:reservoir-s-
      a       owl:Class ;
      rdfs:comment "reservoir(s).  an artificial pond or lake"@en ;
      rdfs:subClassOf ontologyofspatialobject:Hydrographic .

ontologyofspatialobject:ferry
      a       owl:Class ;
      rdfs:comment "ferry.  a boat or other floating conveyance and terminal facilities regularly used to transport people and vehicles across a waterbody"@en ;
      rdfs:subClassOf ontologyofspatialobject:Spot .

ontologyofspatialobject:estuary
      a       owl:Class ;
      rdfs:comment "estuary.  a funnel-shaped stream mouth or embayment where fresh water mixes with sea water under tidal influences"@en ;
      rdfs:subClassOf ontologyofspatialobject:Hydrographic .

ontologyofspatialobject:stable
      a       owl:Class ;
      rdfs:comment "stable.  a building for the shelter and feeding of farm animals, especially horses"@en ;
      rdfs:subClassOf ontologyofspatialobject:Spot .

ontologyofspatialobject:racetrack
      a       owl:Class ;
      rdfs:comment "racetrack.  a track where races are held"@en ;
      rdfs:subClassOf ontologyofspatialobject:Spot .

ontologyofspatialobject:interdune-trough-s-
      a       owl:Class ;
      rdfs:comment "interdune trough(s).  a long wind-swept trough between parallel longitudinal dunes"@en ;
      rdfs:subClassOf ontologyofspatialobject:Hypsographic .

ontologyofspatialobject:Barriers-on-waterways
      a       owl:Class ;
      rdfs:subClassOf ontologyofspatialobject:Hydrographic .

ontologyofspatialobject:estate-s-
      a       owl:Class ;
      rdfs:comment "estate(s).  a large commercialized agricultural landholding with associated buildings and other facilities"@en ;
      rdfs:subClassOf ontologyofspatialobject:Spot .

ontologyofspatialobject:sabkha-s-
      a       owl:Class ;
      rdfs:comment "sabkha(s).  a salt flat or salt encrusted plain subject to periodic inundation from flooding or high tides"@en ;
      rdfs:subClassOf ontologyofspatialobject:Hydrographic .

ontologyofspatialobject:hills
      a       owl:Class ;
      rdfs:comment "hills.  elevations rising generally less than 500 meters"@en , "hills.  rounded elevations of limited extent rising above the surrounding land with local relief of less than 300m"@en ;
      rdfs:subClassOf ontologyofspatialobject:Hypsographic , ontologyofspatialobject:Undersea .

ontologyofspatialobject:sill
      a       owl:Class ;
      rdfs:comment "sill.  the low part of an underwater gap or saddle separating basins, including a similar feature at the mouth of a fjord"@en , "sill.  the low part of a gap or saddle separating basins"@en ;
      rdfs:subClassOf ontologyofspatialobject:Hydrographic , ontologyofspatialobject:Undersea .

ontologyofspatialobject:touches
      a       owl:ObjectProperty , owl:SymmetricProperty ;
      rdfs:comment """Two geometries touch if the intersection of their interiors is empty, but the intersection of the two geometries is not empty.

http://esri.github.io/geometry-api-java/doc/Touches.html"""@en ;
      rdfs:domain ontologyofspatialobject:SpatialObject ;
      rdfs:range ontologyofspatialobject:SpatialObject ;
      rdfs:subPropertyOf ontologyofspatialobject:topological .

ontologyofspatialobject:common
      a       owl:Class ;
      rdfs:comment "common.  a park or pasture for community use"@en ;
      rdfs:subClassOf ontologyofspatialobject:Area .

ontologyofspatialobject:water-mill
      a       owl:Class ;
      rdfs:comment "water mill.  a mill powered by running water"@en ;
      rdfs:subClassOf ontologyofspatialobject:Spot .

ontologyofspatialobject:abandoned-airfield
      a       owl:Class ;
      rdfs:comment "abandoned airfield.  "@en ;
      rdfs:subClassOf ontologyofspatialobject:Spot .

[]    a       owl:AllDisjointProperties ;
      owl:members (ontologyofspatialobject:featureCode ontologyofspatialobject:featureCodeName ontologyofspatialobject:geoNameId ontologyofspatialobject:latitude ontologyofspatialobject:longitude ontologyofspatialobject:timezone ontologyofspatialobject:wkt) .

ontologyofspatialobject:waterworks
      a       owl:Class ;
      rdfs:comment "waterworks.  a facility for supplying potable water through a water source and a system of pumps and filtration beds"@en ;
      rdfs:subClassOf ontologyofspatialobject:Spot .

ontologyofspatialobject:wadies
      a       owl:Class ;
      rdfs:comment "wadies.   found primarily in North Africa and the Middle East\""@en ;
      rdfs:subClassOf ontologyofspatialobject:Hydrographic .

owl:preferredNamespacePrefix
      a       owl:AnnotationProperty .

ontologyofspatialobject:wadi-mouth
      a       owl:Class ;
      rdfs:comment "wadi mouth.  the lower terminus of a wadi where it widens into an adjoining floodplain, depression, or waterbody"@en ;
      rdfs:subClassOf ontologyofspatialobject:Hydrographic .

ontologyofspatialobject:theater
      a       owl:Class ;
      rdfs:comment "theater.  A building, room, or outdoor structure for the presentation of plays, films, or other dramatic performances"@en ;
      rdfs:subClassOf ontologyofspatialobject:Spot .

ontologyofspatialobject:research-institute
      a       owl:Class ;
      rdfs:comment "research institute.  a facility where research is carried out"@en ;
      rdfs:subClassOf ontologyofspatialobject:Spot .

ontologyofspatialobject:intermittent-pond
      a       owl:Class ;
      rdfs:comment "intermittent pond.  "@en ;
      rdfs:subClassOf ontologyofspatialobject:Hydrographic .

ontologyofspatialobject:typeRelation
      a       owl:FunctionalProperty , owl:DatatypeProperty ;
      rdfs:comment "Define el tipo de relacion entre los elementos de la Relacion"@es ;
      rdfs:domain ontologyofspatialobject:SpatialObject ;
      rdfs:range xsd:string ;
      rdfs:subPropertyOf ontologyofspatialobject:osmDataProperty .

ontologyofspatialobject:Area
      a       owl:Class ;
      rdfs:comment "L parks,area, ..."@en ;
      rdfs:subClassOf ontologyofspatialobject:GeonameConcept .

ontologyofspatialobject:plain
      a       owl:Class ;
      rdfs:comment "plain.  a flat, gently sloping or nearly level region"@en ;
      rdfs:subClassOf ontologyofspatialobject:Undersea .

ontologyofspatialobject:quay
      a       owl:Class ;
      rdfs:comment "quay.  a structure of solid construction along a shore or bank which provides berthing for ships and which generally provides cargo handling facilities"@en ;
      rdfs:subClassOf ontologyofspatialobject:Spot .

ontologyofspatialobject:free-trade-zone
      a       owl:Class ;
      rdfs:comment "free trade zone.  an area, usually a section of a port, where goods may be received and shipped free of customs duty and of most customs regulations"@en ;
      rdfs:subClassOf ontologyofspatialobject:Spot .

ontologyofspatialobject:boatyard
      a       owl:Class ;
      rdfs:comment "boatyard.  a waterside facility for servicing, repairing, and building small vessels"@en ;
      rdfs:subClassOf ontologyofspatialobject:Spot .

ontologyofspatialobject:landfill
      a       owl:Class ;
      rdfs:comment "landfill.  a place for trash and garbage disposal in which the waste is buried between layers of earth to build up low-lying land"@en ;
      rdfs:subClassOf ontologyofspatialobject:Spot .

ontologyofspatialobject:agricultural-facility
      a       owl:Class ;
      rdfs:comment "agricultural facility.  a building and/or tract of land used for improving agriculture"@en ;
      rdfs:subClassOf ontologyofspatialobject:Spot .

ontologyofspatialobject:lighthouse
      a       owl:Class ;
      rdfs:comment "lighthouse.  a distinctive structure exhibiting a major navigation light"@en ;
      rdfs:subClassOf ontologyofspatialobject:Spot .

ontologyofspatialobject:natural
      a       owl:Class ;
      rdfs:comment "This is used to describe natural and physical land features. These also include features that have been modified by humans. See the page titled Natural(\"http://wiki.openstreetmap.org/wiki/Natural\") for an introduction on its usage. "@en ;
      rdfs:subClassOf ontologyofspatialobject:SpatialObject .

ontologyofspatialobject:gate
      a       owl:Class ;
      rdfs:comment "gate.  a controlled access entrance or exit"@en ;
      rdfs:subClassOf ontologyofspatialobject:Spot .

ontologyofspatialobject:lagoon
      a       owl:Class ;
      rdfs:comment "lagoon.  a shallow coastal waterbody, completely or partly separated from a larger body of water by a barrier island, coral reef or other depositional feature"@en ;
      rdfs:subClassOf ontologyofspatialobject:Natural-watercourses , ontologyofspatialobject:Hydrographic .

ontologyofspatialobject:wadi-junction
      a       owl:Class ;
      rdfs:comment "wadi junction.  a place where two or more wadies join"@en ;
      rdfs:subClassOf ontologyofspatialobject:Hydrographic .

ontologyofspatialobject:hunting-reserve
      a       owl:Class ;
      rdfs:comment "hunting reserve.  a tract of land used primarily for hunting"@en ;
      rdfs:subClassOf ontologyofspatialobject:Area .

ontologyofspatialobject:intermittent-salt-lake
      a       owl:Class ;
      rdfs:comment "intermittent salt lake.  "@en ;
      rdfs:subClassOf ontologyofspatialobject:Hydrographic .

ontologyofspatialobject:logging-camp
      a       owl:Class ;
      rdfs:comment "logging camp.  a camp used by loggers"@en ;
      rdfs:subClassOf ontologyofspatialobject:Spot .

ontologyofspatialobject:oasis--es-
      a       owl:Class ;
      rdfs:comment "oasis(-es).  an area in a desert made productive by the availability of water"@en ;
      rdfs:subClassOf ontologyofspatialobject:Area .

[]    a       owl:AllDisjointProperties ;
      owl:members (ontologyofspatialobject:adminName3 ontologyofspatialobject:elevation ontologyofspatialobject:rank ontologyofspatialobject:thumbnailImg ontologyofspatialobject:timezone ontologyofspatialobject:wikipediaUrl ontologyofspatialobject:wkt) .

ontologyofspatialobject:pinnacle
      a       owl:Class ;
      rdfs:comment "pinnacle.  a high tower or spire-shaped pillar of rock or coral, alone or cresting a summit"@en ;
      rdfs:subClassOf ontologyofspatialobject:Undersea .

ontologyofspatialobject:bus-station
      a       owl:Class ;
      rdfs:comment "bus station.  a facility comprising ticket office, platforms, etc. for loading and unloading passengers"@en ;
      rdfs:subClassOf ontologyofspatialobject:Spot .

ontologyofspatialobject:palm-grove
      a       owl:Class ;
      rdfs:comment "palm grove.  a planting of palm trees"@en ;
      rdfs:subClassOf ontologyofspatialobject:Vegetation .

ontologyofspatialobject:roadstead
      a       owl:Class ;
      rdfs:comment "roadstead.  an open anchorage affording less protection than a harbor"@en ;
      rdfs:subClassOf ontologyofspatialobject:Hydrographic .

ontologyofspatialobject:concession-area
      a       owl:Class ;
      rdfs:comment "concession area.  a lease of land by a government for economic development, e.g., mining, forestry"@en ;
      rdfs:subClassOf ontologyofspatialobject:Area .

ontologyofspatialobject:streams
      a       owl:Class ;
      rdfs:comment "streams.  bodies of running water moving to a lower level in a channel on land"@en ;
      rdfs:subClassOf ontologyofspatialobject:Natural-watercourses , ontologyofspatialobject:Hydrographic .

owl:description
      a       owl:AnnotationProperty .

ontologyofspatialobject:mound
      a       owl:Class ;
      rdfs:comment "mound.  a low, isolated, rounded hill"@en ;
      rdfs:subClassOf ontologyofspatialobject:Undersea .

ontologyofspatialobject:continental-rise
      a       owl:Class ;
      rdfs:comment "continental rise.  a gentle slope rising from oceanic depths towards the foot of a continental slope"@en ;
      rdfs:subClassOf ontologyofspatialobject:Undersea .

ontologyofspatialobject:shelf
      a       owl:Class ;
      rdfs:comment "shelf.  a zone adjacent to a continent (or around an island) that extends from the low water line to a depth at which there is usually a marked increase of slope towards oceanic depths"@en ;
      rdfs:subClassOf ontologyofspatialobject:Undersea .

ontologyofspatialobject:waterhole-s-
      a       owl:Class ;
      rdfs:comment "waterhole(s).  a natural hole, hollow, or small depression that contains water, used by man and animals, especially in arid areas"@en ;
      rdfs:subClassOf ontologyofspatialobject:Hydrographic .

ontologyofspatialobject:oil-pipeline-terminal
      a       owl:Class ;
      rdfs:comment "oil pipeline terminal.  a tank farm or loading facility at the end of an oil pipeline"@en ;
      rdfs:subClassOf ontologyofspatialobject:Spot .

ontologyofspatialobject:limekiln
      a       owl:Class ;
      rdfs:comment "limekiln.  a furnace in which limestone is reduced to lime"@en ;
      rdfs:subClassOf ontologyofspatialobject:Spot .

[]    a       owl:AllDisjointProperties ;
      owl:members (ontologyofspatialobject:adminName5 ontologyofspatialobject:elevation ontologyofspatialobject:language ontologyofspatialobject:latitude ontologyofspatialobject:longitude ontologyofspatialobject:rank ontologyofspatialobject:summary ontologyofspatialobject:thumbnailImg ontologyofspatialobject:wikipediaUrl ontologyofspatialobject:wkt) .

rdfs:comment
      rdfs:comment "This ontology is designed to model any geographical area."@en .

ontologyofspatialobject:adminCode4
      a       owl:FunctionalProperty , owl:DatatypeProperty ;
      rdfs:comment "adminCode4"@en ;
      rdfs:domain ontologyofspatialobject:SpatialObject ;
      rdfs:range xsd:string ;
      rdfs:subPropertyOf ontologyofspatialobject:gonameDataProperty .

ontologyofspatialobject:GeonameConcept
      a       owl:Class ;
      rdfs:comment "Geoname Concept"@en ;
      rdfs:subClassOf ontologyofspatialobject:SpatialObject .

ontologyofspatialobject:house-s-
      a       owl:Class ;
      rdfs:comment "house(s).  a building used as a human habitation"@en ;
      rdfs:subClassOf ontologyofspatialobject:Spot .

ontologyofspatialobject:farm-village
      a       owl:Class ;
      rdfs:comment "farm village.  a populated place where the population is largely engaged in agricultural activities"@en ;
      rdfs:subClassOf ontologyofspatialobject:PopulatedPlace .

ontologyofspatialobject:islet
      a       owl:Class ;
      rdfs:comment "islet.  small island, bigger than rock, smaller than island."@en ;
      rdfs:subClassOf ontologyofspatialobject:Hypsographic .

ontologyofspatialobject:trail
      a       owl:Class ;
      rdfs:comment "trail.  a path, track, or route used by pedestrians, animals, or off-road vehicles"@en ;
      rdfs:subClassOf ontologyofspatialobject:Road .

ontologyofspatialobject:sugar-plantation
      a       owl:Class ;
      rdfs:comment "sugar plantation.  an estate that specializes in growing sugar cane"@en ;
      rdfs:subClassOf ontologyofspatialobject:Spot .

ontologyofspatialobject:customs-house
      a       owl:Class ;
      rdfs:comment "customs house.  a building in a port where customs and duties are paid, and where vessels are entered and cleared"@en ;
      rdfs:subClassOf ontologyofspatialobject:Spot .

ontologyofspatialobject:stock-route
      a       owl:Class ;
      rdfs:comment "stock route.  a route taken by livestock herds"@en ;
      rdfs:subClassOf ontologyofspatialobject:Road .

ontologyofspatialobject:store
      a       owl:Class ;
      rdfs:comment "store.  a building where goods and/or services are offered for sale"@en ;
      rdfs:subClassOf ontologyofspatialobject:Spot .

ontologyofspatialobject:adminCode3
      a       owl:FunctionalProperty , owl:DatatypeProperty ;
      rdfs:comment "adminCode3"@en ;
      rdfs:domain ontologyofspatialobject:SpatialObject ;
      rdfs:range xsd:string ;
      rdfs:subPropertyOf ontologyofspatialobject:gonameDataProperty .

ontologyofspatialobject:building
      a       owl:Class ;
      rdfs:comment "This is used to identify individual buildings or groups of connected buildings. See the page Building(\"http://wiki.openstreetmap.org/wiki/Buildings\") for further details on the usage of this tag"@en ;
      rdfs:subClassOf ontologyofspatialobject:Spot .

ontologyofspatialobject:drainage-ditch
      a       owl:Class ;
      rdfs:comment "drainage ditch.  a ditch which serves to drain the land"@en ;
      rdfs:subClassOf ontologyofspatialobject:Man-made-waterways , ontologyofspatialobject:Hydrographic .

ontologyofspatialobject:dispensary
      a       owl:Class ;
      rdfs:comment "dispensary.  a building where medical or dental aid is dispensed"@en ;
      rdfs:subClassOf ontologyofspatialobject:Spot .

ontologyofspatialobject:ditch-mouth-s-
      a       owl:Class ;
      rdfs:comment "ditch mouth(s).  an area where a drainage ditch enters a lagoon, lake or bay"@en ;
      rdfs:subClassOf ontologyofspatialobject:Hydrographic .

ontologyofspatialobject:fifth-order-administrative-division
      a       owl:Class ;
      rdfs:comment "fifth-order administrative division.  a subdivision of a fourth-order administrative division"@en ;
      rdfs:subClassOf ontologyofspatialobject:AdministrativeBoundary .

ontologyofspatialobject:cattle-dipping-tank
      a       owl:Class ;
      rdfs:comment "cattle dipping tank.  a small artificial pond used for immersing cattle in chemically treated water for disease control"@en ;
      rdfs:subClassOf ontologyofspatialobject:Spot .

ontologyofspatialobject:water-tank
      a       owl:Class ;
      rdfs:comment "water tank.  a contained pool or tank of water at, below, or above ground level"@en ;
      rdfs:subClassOf ontologyofspatialobject:Hydrographic .

ontologyofspatialobject:artificial-island
      a       owl:Class ;
      rdfs:comment "artificial island.  an island created by landfill or diking and filling in a wetland, bay, or lagoon"@en ;
      rdfs:subClassOf ontologyofspatialobject:Hypsographic .

ontologyofspatialobject:corridor
      a       owl:Class ;
      rdfs:comment "corridor.  a strip or area of land having significance as an access way"@en ;
      rdfs:subClassOf ontologyofspatialobject:Hypsographic .

ontologyofspatialobject:isNearOf
      a       owl:ObjectProperty , owl:SymmetricProperty , owl:ReflexiveProperty ;
      rdfs:comment "Is near of"@en ;
      rdfs:domain ontologyofspatialobject:SpatialObject ;
      rdfs:range ontologyofspatialobject:SpatialObject ;
      rdfs:subPropertyOf ontologyofspatialobject:proximity .

ontologyofspatialobject:golf-course
      a       owl:Class ;
      rdfs:comment "golf course.  a recreation field where golf is played"@en ;
      rdfs:subClassOf ontologyofspatialobject:Spot .

ontologyofspatialobject:military-installation
      a       owl:Class ;
      rdfs:comment "military installation.  a facility for use of and control by armed forces"@en ;
      rdfs:subClassOf ontologyofspatialobject:Spot .

ontologyofspatialobject:osmDataProperty
      a       owl:DatatypeProperty ;
      rdfs:comment "Se reutilizan los siguientes dataproperty de Geoname: longitud, latitud"@es ;
      rdfs:domain ontologyofspatialobject:SpatialObject ;
      rdfs:range rdfs:Literal ;
      rdfs:subPropertyOf owl:topDataProperty .

ontologyofspatialobject:coconut-grove
      a       owl:Class ;
      rdfs:comment "coconut grove.  a planting of coconut trees"@en ;
      rdfs:subClassOf ontologyofspatialobject:Vegetation .

ontologyofspatialobject:arctic-land
      a       owl:Class ;
      rdfs:comment "arctic land.  a tract of land in the Arctic"@en ;
      rdfs:subClassOf ontologyofspatialobject:Area .

[]    a       owl:AllDisjointProperties ;
      owl:members (ontologyofspatialobject:alternateNames ontologyofspatialobject:boundingBox ontologyofspatialobject:elevation) .

ontologyofspatialobject:beach
      a       owl:Class ;
      rdfs:comment "beach.  a shore zone of coarse unconsolidated sediment that extends from the low-water line to the highest reach of storm waves"@en ;
      rdfs:subClassOf ontologyofspatialobject:Hypsographic .

ontologyofspatialobject:swamp
      a       owl:Class ;
      rdfs:comment "swamp.  a wetland dominated by tree vegetation"@en ;
      rdfs:subClassOf ontologyofspatialobject:Hydrographic .

ontologyofspatialobject:aquaculture-facility
      a       owl:Class ;
      rdfs:comment "aquaculture facility.   underwater agriculture\""@en ;
      rdfs:subClassOf ontologyofspatialobject:Spot .

ontologyofspatialobject:aqueduct
      a       owl:Class ;
      rdfs:comment "aqueduct.  a conduit used to carry water"@en ;
      rdfs:subClassOf ontologyofspatialobject:Man-made-waterways , ontologyofspatialobject:Hydrographic .

ontologyofspatialobject:space-center
      a       owl:Class ;
      rdfs:comment "space center.  a facility for launching, tracking, or controlling satellites and space vehicles"@en ;
      rdfs:subClassOf ontologyofspatialobject:Spot .

ontologyofspatialobject:terrace
      a       owl:Class ;
      rdfs:comment "terrace.  a long, narrow alluvial platform bounded by steeper slopes above and below, usually overlooking a waterbody"@en , "terrace.  a relatively flat horizontal or gently inclined surface, sometimes long and narrow, which is bounded by a steeper ascending slope on one side and by a steep descending slope on the opposite side"@en ;
      rdfs:subClassOf ontologyofspatialobject:Hypsographic , ontologyofspatialobject:Undersea .

ontologyofspatialobject:confluence
      a       owl:Class ;
      rdfs:comment "confluence.  a place where two or more streams or intermittent streams flow together"@en ;
      rdfs:subClassOf ontologyofspatialobject:Hydrographic .

ontologyofspatialobject:crosses
      a       owl:ObjectProperty , owl:SymmetricProperty ;
      rdfs:comment """Two polylines cross if they meet at points only, and at least one of the shared points is internal to both polylines. A polyline and polygon cross if a connected part of the polyline is partly inside and partly outside the polygon.

http://esri.github.io/geometry-api-java/doc/Crosses.html"""@en ;
      rdfs:domain ontologyofspatialobject:SpatialObject ;
      rdfs:range ontologyofspatialobject:SpatialObject ;
      rdfs:subPropertyOf ontologyofspatialobject:topological ;
      owl:propertyDisjointWith
              ontologyofspatialobject:disjoint , ontologyofspatialobject:equal .

ontologyofspatialobject:ford
      a       owl:Class ;
      rdfs:comment "ford.  a shallow part of a stream which can be crossed on foot or by land vehicle"@en ;
      rdfs:subClassOf ontologyofspatialobject:Hypsographic .

ontologyofspatialobject:adminCode5
      a       owl:FunctionalProperty , owl:DatatypeProperty ;
      rdfs:comment "adminCode5"@en ;
      rdfs:domain ontologyofspatialobject:SpatialObject ;
      rdfs:range xsd:string ;
      rdfs:subPropertyOf ontologyofspatialobject:gonameDataProperty .

ontologyofspatialobject:baling-station
      a       owl:Class ;
      rdfs:comment "baling station.  a facility for baling agricultural products"@en ;
      rdfs:subClassOf ontologyofspatialobject:Spot .

ontologyofspatialobject:spur-s-
      a       owl:Class ;
      rdfs:comment "spur(s).  a subordinate ridge projecting outward from a hill, mountain or other elevation"@en ;
      rdfs:subClassOf ontologyofspatialobject:Hypsographic .

[]    a       swrl:Imp ;
      swrl:body
              [ a       swrl:AtomList ;
                rdf:first
                        [ a       swrl:BuiltinAtom ;
                          swrl:arguments
                                  [ a       rdf:List ;
                                    rdf:first <urn:swrl#latitud> ;
                                    rdf:rest
                                            [ a       rdf:List ;
                                              rdf:first 0 ;
                                              rdf:rest ()
                                            ]
                                  ] ;
                          swrl:builtin swrlb:lessThan
                        ] ;
                rdf:rest
                        [ a       swrl:AtomList ;
                          rdf:first
                                  [ a       swrl:DatavaluedPropertyAtom ;
                                    swrl:argument1 <urn:swrl#x> ;
                                    swrl:argument2 <urn:swrl#latitud> ;
                                    swrl:propertyPredicate
                                            ontologyofspatialobject:latitude
                                  ] ;
                          rdf:rest
                                  [ a       swrl:AtomList ;
                                    rdf:first
                                            [ a       swrl:ClassAtom ;
                                              swrl:argument1 <urn:swrl#x> ;
                                              swrl:classPredicate ontologyofspatialobject:SpatialObject
                                            ] ;
                                    rdf:rest ()
                                  ]
                        ]
              ] ;
      swrl:head
              [ a       swrl:AtomList ;
                rdf:first
                        [ a       swrl:ClassAtom ;
                          swrl:argument1 <urn:swrl#x> ;
                          swrl:classPredicate ontologyofspatialobject:SurtHemisphere
                        ] ;
                rdf:rest ()
              ] .

ontologyofspatialobject:community-center
      a       owl:Class ;
      rdfs:comment "community center.  a facility for community recreation and other activities"@en ;
      rdfs:subClassOf ontologyofspatialobject:Spot .

ontologyofspatialobject:triangulation-station
      a       owl:Class ;
      rdfs:comment "triangulation station.  a point on the earth whose position has been determined by triangulation"@en ;
      rdfs:subClassOf ontologyofspatialobject:Spot .

ontologyofspatialobject:language-school
      a       owl:Class ;
      rdfs:comment "language school.  Language Schools & Institutions"@en ;
      rdfs:subClassOf ontologyofspatialobject:Spot .

ontologyofspatialobject:amusement-park
      a       owl:Class ;
      rdfs:comment "amusement park.  Amusement Park are theme parks, adventure parks offering entertainment, similar to funfairs but with a fix location"@en ;
      rdfs:subClassOf ontologyofspatialobject:Area .

ontologyofspatialobject:creators
      a       owl:AnnotationProperty .

ontologyofspatialobject:wetland
      a       owl:Class ;
      rdfs:comment "wetland.  an area subject to inundation, usually characterized by bog, marsh, or swamp vegetation"@en ;
      rdfs:subClassOf ontologyofspatialobject:Hydrographic .

ontologyofspatialobject:snowfield
      a       owl:Class ;
      rdfs:comment "snowfield.  an area of permanent snow and ice forming the accumulation area of a glacier"@en ;
      rdfs:subClassOf ontologyofspatialobject:Area .

ontologyofspatialobject:latitude
      a       owl:FunctionalProperty , owl:DatatypeProperty ;
      rdfs:comment "Es utilizada por Geonames, OSM y por Wikipedia" ;
      rdfs:domain ontologyofspatialobject:SpatialObject ;
      rdfs:range xsd:double ;
      rdfs:subPropertyOf owl:topDataProperty .

ontologyofspatialobject:ancient-wall
      a       owl:Class ;
      rdfs:comment "ancient wall.  the remains of a linear defensive stone structure"@en ;
      rdfs:subClassOf ontologyofspatialobject:Spot .

ontologyofspatialobject:promenade
      a       owl:Class ;
      rdfs:comment "promenade.  a place for public walking, usually along a beach front"@en ;
      rdfs:subClassOf ontologyofspatialobject:Road .

ontologyofspatialobject:building-s-
      a       owl:Class ;
      rdfs:comment "building(s).  a structure built for permanent use, as a house, factory, etc."@en ;
      rdfs:subClassOf ontologyofspatialobject:Spot .

ontologyofspatialobject:church
      a       owl:Class ;
      rdfs:comment "church.  a building for public Christian worship"@en ;
      rdfs:subClassOf ontologyofspatialobject:Spot .

ontologyofspatialobject:tea-plantation
      a       owl:Class ;
      rdfs:comment "tea plantation.  an estate which specializes in growing tea bushes"@en ;
      rdfs:subClassOf ontologyofspatialobject:Spot .

ontologyofspatialobject:power-station
      a       owl:Class ;
      rdfs:comment "power station.  a facility for generating electric power"@en ;
      rdfs:subClassOf ontologyofspatialobject:Spot .

[]    a       owl:AllDisjointProperties ;
      owl:members (ontologyofspatialobject:adminCode1 ontologyofspatialobject:adminCode2 ontologyofspatialobject:adminCode3 ontologyofspatialobject:adminCode4 ontologyofspatialobject:adminCode5 ontologyofspatialobject:adminName1 ontologyofspatialobject:adminName2 ontologyofspatialobject:adminName3 ontologyofspatialobject:adminName4 ontologyofspatialobject:adminName5 ontologyofspatialobject:language ontologyofspatialobject:population ontologyofspatialobject:typeRelation ontologyofspatialobject:wkt) .

ontologyofspatialobject:oil-well
      a       owl:Class ;
      rdfs:comment "oil well.  a well from which oil may be pumped"@en ;
      rdfs:subClassOf ontologyofspatialobject:Spot .

ontologyofspatialobject:pond
      a       owl:Class ;
      rdfs:comment "pond.  a small standing waterbody"@en ;
      rdfs:subClassOf ontologyofspatialobject:Hydrographic .

ontologyofspatialobject:wall
      a       owl:Class ;
      rdfs:comment "wall.  a thick masonry structure, usually enclosing a field or building, or forming the side of a structure"@en ;
      rdfs:subClassOf ontologyofspatialobject:Spot .

ontologyofspatialobject:gully
      a       owl:Class ;
      rdfs:comment "gully.  a small valley-like feature"@en ;
      rdfs:subClassOf ontologyofspatialobject:Undersea .

ontologyofspatialobject:icecap-ridge
      a       owl:Class ;
      rdfs:comment "icecap ridge.  a linear elevation on an icecap"@en ;
      rdfs:subClassOf ontologyofspatialobject:Hydrographic .

ontologyofspatialobject:economic-region
      a       owl:Class ;
      rdfs:comment "economic region.  a region of a country established for economic development or for statistical purposes"@en ;
      rdfs:subClassOf ontologyofspatialobject:Area .

ontologyofspatialobject:meander-neck
      a       owl:Class ;
      rdfs:comment "meander neck.  a narrow strip of land between the two limbs of a meander loop at its narrowest point"@en ;
      rdfs:subClassOf ontologyofspatialobject:Hypsographic .

ontologyofspatialobject:marine-channel
      a       owl:Class ;
      rdfs:comment "marine channel.  that part of a body of water deep enough for navigation through an area otherwise not suitable"@en ;
      rdfs:subClassOf ontologyofspatialobject:Hydrographic .

ontologyofspatialobject:section-of-island
      a       owl:Class ;
      rdfs:comment "section of island.  "@en ;
      rdfs:subClassOf ontologyofspatialobject:Hypsographic .

ontologyofspatialobject:butte-s-
      a       owl:Class ;
      rdfs:comment "butte(s).  a small, isolated, usually flat-topped hill with steep sides"@en ;
      rdfs:subClassOf ontologyofspatialobject:Hypsographic .

ontologyofspatialobject:hole
      a       owl:Class ;
      rdfs:comment "hole.  a small depression of the sea floor"@en ;
      rdfs:subClassOf ontologyofspatialobject:Undersea .

ontologyofspatialobject:ridge
      a       owl:Class ;
      rdfs:comment "ridge.  a long narrow elevation with steep sides"@en ;
      rdfs:subClassOf ontologyofspatialobject:Undersea .

ontologyofspatialobject:elevation
      a       owl:FunctionalProperty , owl:DatatypeProperty ;
      rdfs:comment """the elevation in metres (optional may be null), parsed from the article or reverse geocoded.

Es utilizada por Geonames y por Wikipedia"""@en ;
      rdfs:domain ontologyofspatialobject:SpatialObject ;
      rdfs:range xsd:integer ;
      rdfs:subPropertyOf owl:topDataProperty .

ontologyofspatialobject:blowhole-s-
      a       owl:Class ;
      rdfs:comment "blowhole(s).  a hole in coastal rock through which sea water is forced by a rising tide or waves and spurted through an outlet into the air"@en ;
      rdfs:subClassOf ontologyofspatialobject:Hypsographic .

ontologyofspatialobject:sub-surface-dam
      a       owl:Class ;
      rdfs:comment "sub-surface dam.  a dam put down to bedrock in a sand river"@en ;
      rdfs:subClassOf ontologyofspatialobject:Spot .

ontologyofspatialobject:lake-bed-s-
      a       owl:Class ;
      rdfs:comment "lake bed(s).  a dried up or drained area of a former lake"@en ;
      rdfs:subClassOf ontologyofspatialobject:Hydrographic .

ontologyofspatialobject:locality
      a       owl:Class ;
      rdfs:comment "locality.  a minor area or place of unspecified or mixed character and indefinite boundaries"@en ;
      rdfs:subClassOf ontologyofspatialobject:Area .

ontologyofspatialobject:idOSM
      a       owl:FunctionalProperty , owl:DatatypeProperty ;
      rdfs:comment "Es el id de los objetos de OSM. Pudo haberse trabajado con el mismo dataproperty id de Geoname (geoNameId) pero no se hizo."@es ;
      rdfs:domain ontologyofspatialobject:SpatialObject ;
      rdfs:range xsd:unsignedLong ;
      rdfs:subPropertyOf ontologyofspatialobject:osmDataProperty .

ontologyofspatialobject:road-cut
      a       owl:Class ;
      rdfs:comment "road cut.  an excavation cut through a hill or ridge for a road"@en ;
      rdfs:subClassOf ontologyofspatialobject:Road .

ontologyofspatialobject:adminCode2
      a       owl:FunctionalProperty , owl:DatatypeProperty ;
      rdfs:comment "adminCode2"@en ;
      rdfs:domain ontologyofspatialobject:SpatialObject ;
      rdfs:range xsd:string ;
      rdfs:subPropertyOf ontologyofspatialobject:gonameDataProperty .

ontologyofspatialobject:navigation-canal-s-
      a       owl:Class ;
      rdfs:comment "navigation canal(s).  a watercourse constructed for navigation of vessels"@en ;
      rdfs:subClassOf ontologyofspatialobject:Hydrographic .

ontologyofspatialobject:rookery
      a       owl:Class ;
      rdfs:comment "rookery.  a breeding place of a colony of birds or seals"@en ;
      rdfs:subClassOf ontologyofspatialobject:Spot .

ontologyofspatialobject:boulder-field
      a       owl:Class ;
      rdfs:comment "boulder field.  a high altitude or high latitude bare, flat area covered with large angular rocks"@en ;
      rdfs:subClassOf ontologyofspatialobject:Hypsographic .

ontologyofspatialobject:section-of-intermittent-stream
      a       owl:Class ;
      rdfs:comment "section of intermittent stream.  "@en ;
      rdfs:subClassOf ontologyofspatialobject:Hydrographic .

ontologyofspatialobject:caldera
      a       owl:Class ;
      rdfs:comment "caldera.  a depression measuring kilometers across formed by the collapse of a volcanic mountain"@en ;
      rdfs:subClassOf ontologyofspatialobject:Hypsographic .

ontologyofspatialobject:inspection-station
      a       owl:Class ;
      rdfs:comment "inspection station.  a station at which vehicles, goods, and people are inspected"@en ;
      rdfs:subClassOf ontologyofspatialobject:Spot .

ontologyofspatialobject:irrigation-system
      a       owl:Class ;
      rdfs:comment "irrigation system.  a network of ditches and one or more of the following elements: water supply, reservoir, canal, pump, well, drain, etc."@en ;
      rdfs:subClassOf ontologyofspatialobject:Hydrographic .

ontologyofspatialobject:airfield
      a       owl:Class ;
      rdfs:comment "airfield.   no facilities provided for the commercial handling of passengers and cargo\""@en ;
      rdfs:subClassOf ontologyofspatialobject:Spot .

ontologyofspatialobject:capital-of-a-political-entity
      a       owl:Class ;
      rdfs:comment "capital of a political entity.  "@en ;
      rdfs:subClassOf ontologyofspatialobject:PopulatedPlace .

ontologyofspatialobject:independent-political-entity
      a       owl:Class ;
      rdfs:comment "independent political entity.  "@en ;
      rdfs:subClassOf ontologyofspatialobject:AdministrativeBoundary .

ontologyofspatialobject:pass
      a       owl:Class ;
      rdfs:comment "pass.  a break in a mountain range or other high obstruction, used for transportation from one side to the other [See also gap]"@en ;
      rdfs:subClassOf ontologyofspatialobject:Hypsographic .

ontologyofspatialobject:ghat
      a       owl:Class ;
      rdfs:comment "ghat.  a set of steps leading to a river, which are of religious significance, and at their base is usually a platform for bathing"@en ;
      rdfs:subClassOf ontologyofspatialobject:Spot .

ontologyofspatialobject:country-house
      a       owl:Class ;
      rdfs:comment "country house.  a large house, mansion, or chateau, on a large estate"@en ;
      rdfs:subClassOf ontologyofspatialobject:Spot .

ontologyofspatialobject:cultivated-area
      a       owl:Class ;
      rdfs:comment "cultivated area.  an area under cultivation"@en ;
      rdfs:subClassOf ontologyofspatialobject:Vegetation .

ontologyofspatialobject:adminCode1
      a       owl:FunctionalProperty , owl:DatatypeProperty ;
      rdfs:comment "adminCode1"@en ;
      rdfs:domain ontologyofspatialobject:SpatialObject ;
      rdfs:range xsd:string ;
      rdfs:subPropertyOf ontologyofspatialobject:gonameDataProperty .

ontologyofspatialobject:geoNameId
      a       owl:FunctionalProperty , owl:DatatypeProperty ;
      rdfs:comment "geonameId"@en ;
      rdfs:domain ontologyofspatialobject:SpatialObject ;
      rdfs:range xsd:int ;
      rdfs:subPropertyOf ontologyofspatialobject:gonameDataProperty .

ontologyofspatialobject:abandoned-watercourse
      a       owl:Class ;
      rdfs:comment "abandoned watercourse.  a former stream or distributary no longer carrying flowing water, but still evident due to lakes, wetland, topographic or vegetation patterns"@en ;
      rdfs:subClassOf ontologyofspatialobject:Hydrographic .

ontologyofspatialobject:mine-s-
      a       owl:Class ;
      rdfs:comment "mine(s).  a site where mineral ores are extracted from the ground by excavating surface pits and subterranean passages"@en ;
      rdfs:subClassOf ontologyofspatialobject:Spot .

ontologyofspatialobject:upland
      a       owl:Class ;
      rdfs:comment "upland.  an extensive interior region of high land with low to moderate surface relief"@en ;
      rdfs:subClassOf ontologyofspatialobject:Hypsographic .

ontologyofspatialobject:karst-area
      a       owl:Class ;
      rdfs:comment "karst area.  a distinctive landscape developed on soluble rock such as limestone characterized by sinkholes, caves, disappearing streams, and underground drainage"@en ;
      rdfs:subClassOf ontologyofspatialobject:Hypsographic .

ontologyofspatialobject:bight-s-
      a       owl:Class ;
      rdfs:comment "bight(s).  an open body of water forming a slight recession in a coastline"@en ;
      rdfs:subClassOf ontologyofspatialobject:Natural-watercourses , ontologyofspatialobject:Hydrographic .

ontologyofspatialobject:semi-independent-political-entity
      a       owl:Class ;
      rdfs:comment "semi-independent political entity.  "@en ;
      rdfs:subClassOf ontologyofspatialobject:AdministrativeBoundary .

ontologyofspatialobject:heliport
      a       owl:Class ;
      rdfs:comment "heliport.  a place where helicopters land and take off"@en ;
      rdfs:subClassOf ontologyofspatialobject:Spot .

ontologyofspatialobject:facility
      a       owl:Class ;
      rdfs:comment "facility.  a building or buildings housing a center, institute, foundation, hospital, prison, mission, courthouse, etc."@en ;
      rdfs:subClassOf ontologyofspatialobject:Spot .

ontologyofspatialobject:shoal-s-
      a       owl:Class ;
      rdfs:comment "shoal(s).  a surface-navigation hazard composed of unconsolidated material"@en ;
      rdfs:subClassOf ontologyofspatialobject:Hydrographic .

ontologyofspatialobject:Water
      a       owl:Class ;
      rdfs:subClassOf ontologyofspatialobject:natural .

ontologyofspatialobject:salt-lake
      a       owl:Class ;
      rdfs:comment "salt lake.  an inland body of salt water with no outlet"@en ;
      rdfs:subClassOf ontologyofspatialobject:Hydrographic .

ontologyofspatialobject:fjord
      a       owl:Class ;
      rdfs:comment "fjord.  a long, narrow, steep-walled, deep-water arm of the sea at high latitudes, usually along mountainous coasts"@en ;
      rdfs:subClassOf ontologyofspatialobject:Hydrographic .

ontologyofspatialobject:contains
      a       owl:TransitiveProperty , owl:ObjectProperty , owl:ReflexiveProperty ;
      rdfs:comment """Contiene_a

One geometry contains another if the other geometry is a subset of it and their interiors have at least one point in common. Contains is the inverse of Within.

http://esri.github.io/geometry-api-java/doc/Contains.html"""@en ;
      rdfs:domain ontologyofspatialobject:SpatialObject ;
      rdfs:range ontologyofspatialobject:SpatialObject ;
      rdfs:subPropertyOf ontologyofspatialobject:topological ;
      owl:propertyDisjointWith
              ontologyofspatialobject:disjoint .

ontologyofspatialobject:ponds
      a       owl:Class ;
      rdfs:comment "ponds.  small standing waterbodies"@en ;
      rdfs:subClassOf ontologyofspatialobject:Hydrographic .

ontologyofspatialobject:volcano
      a       owl:Class ;
      rdfs:comment "volcano.  a conical elevation composed of volcanic materials with a crater at the top"@en ;
      rdfs:subClassOf ontologyofspatialobject:Hypsographic .

ontologyofspatialobject:sawmill
      a       owl:Class ;
      rdfs:comment "sawmill.  a mill where logs or lumber are sawn to specified shapes and sizes"@en ;
      rdfs:subClassOf ontologyofspatialobject:Spot .

ontologyofspatialobject:gas-oil-separator-plant
      a       owl:Class ;
      rdfs:comment "gas-oil separator plant.  a facility for separating gas from oil"@en ;
      rdfs:subClassOf ontologyofspatialobject:Spot .

ontologyofspatialobject:barracks
      a       owl:Class ;
      rdfs:comment "barracks.  a building for lodging military personnel"@en ;
      rdfs:subClassOf ontologyofspatialobject:Spot .

ontologyofspatialobject:nursery--ies-
      a       owl:Class ;
      rdfs:comment "nursery(-ies).  a place where plants are propagated for transplanting or grafting"@en ;
      rdfs:subClassOf ontologyofspatialobject:Spot .

ontologyofspatialobject:coal-mine-s-
      a       owl:Class ;
      rdfs:comment "coal mine(s).  a mine where coal is extracted"@en ;
      rdfs:subClassOf ontologyofspatialobject:Spot .

ontologyofspatialobject:zone
      a       owl:Class ;
      rdfs:comment "zone.  "@en ;
      rdfs:subClassOf ontologyofspatialobject:AdministrativeBoundary .

ontologyofspatialobject:tower
      a       owl:Class ;
      rdfs:comment "tower.  a high conspicuous structure, typically much higher than its diameter"@en ;
      rdfs:subClassOf ontologyofspatialobject:Spot .

ontologyofspatialobject:cave-s-
      a       owl:Class ;
      rdfs:comment "cave(s).  an underground passageway or chamber, or cavity on the side of a cliff"@en ;
      rdfs:subClassOf ontologyofspatialobject:Spot .

ontologyofspatialobject:storehouse
      a       owl:Class ;
      rdfs:comment "storehouse.  a building for storing goods, especially provisions"@en ;
      rdfs:subClassOf ontologyofspatialobject:Spot .

ontologyofspatialobject:arch
      a       owl:Class ;
      rdfs:comment "arch.  a natural or man-made structure in the form of an arch"@en , "arch.  a low bulge around the southeastern end of the island of Hawaii"@en ;
      rdfs:subClassOf ontologyofspatialobject:Spot , ontologyofspatialobject:Undersea .

ontologyofspatialobject:agricultural-colony
      a       owl:Class ;
      rdfs:comment "agricultural colony.  a tract of land set aside for agricultural settlement"@en ;
      rdfs:subClassOf ontologyofspatialobject:Area .

ontologyofspatialobject:quarry--ies-
      a       owl:Class ;
      rdfs:comment "quarry(-ies).  a surface mine where building stone or gravel and sand, etc. are extracted"@en ;
      rdfs:subClassOf ontologyofspatialobject:Spot .

ontologyofspatialobject:abandoned-railroad-stop
      a       owl:Class ;
      rdfs:comment "abandoned railroad stop.  "@en ;
      rdfs:subClassOf ontologyofspatialobject:Spot .

ontologyofspatialobject:narrows
      a       owl:Class ;
      rdfs:comment "narrows.  a navigable narrow part of a bay, strait, river, etc."@en ;
      rdfs:subClassOf ontologyofspatialobject:Hydrographic .

ontologyofspatialobject:coral-reef-s-
      a       owl:Class ;
      rdfs:comment "coral reef(s).  a surface-navigation hazard composed of coral"@en ;
      rdfs:subClassOf ontologyofspatialobject:Hydrographic .

ontologyofspatialobject:breakwater
      a       owl:Class ;
      rdfs:comment "breakwater.  a structure erected to break the force of waves at the entrance to a harbor or port"@en ;
      rdfs:subClassOf ontologyofspatialobject:Spot .

ontologyofspatialobject:observation-point
      a       owl:Class ;
      rdfs:comment "observation point.  a wildlife or scenic observation point"@en ;
      rdfs:subClassOf ontologyofspatialobject:Spot .

ontologyofspatialobject:depression-s-
      a       owl:Class ;
      rdfs:comment "depression(s).  a low area surrounded by higher land and usually characterized by interior drainage"@en ;
      rdfs:subClassOf ontologyofspatialobject:Hypsographic .

ontologyofspatialobject:gasfield
      a       owl:Class ;
      rdfs:comment "gasfield.  an area containing a subterranean store of natural gas of economic value"@en ;
      rdfs:subClassOf ontologyofspatialobject:Area .

ontologyofspatialobject:banks
      a       owl:Class ;
      rdfs:comment "banks.  elevations, typically located on a shelf, over which the depth of water is relatively shallow but sufficient for safe surface navigation"@en ;
      rdfs:subClassOf ontologyofspatialobject:Undersea .

ontologyofspatialobject:populated-place
      a       owl:Class ;
      rdfs:comment "populated place.  a city, town, village, or other agglomeration of buildings where people live and work"@en ;
      rdfs:subClassOf ontologyofspatialobject:PopulatedPlace .

ontologyofspatialobject:munitions-plant
      a       owl:Class ;
      rdfs:comment "munitions plant.  a factory where ammunition is made"@en ;
      rdfs:subClassOf ontologyofspatialobject:Spot .

ontologyofspatialobject:featureClassName
      a       owl:FunctionalProperty , owl:DatatypeProperty ;
      rdfs:domain ontologyofspatialobject:SpatialObject ;
      rdfs:range xsd:string ;
      rdfs:subPropertyOf ontologyofspatialobject:gonameDataProperty .

ontologyofspatialobject:gap
      a       owl:Class ;
      rdfs:comment "gap.  a narrow break in a ridge or rise"@en , "gap.  a low place in a ridge, not used for transportation"@en ;
      rdfs:subClassOf ontologyofspatialobject:Hypsographic , ontologyofspatialobject:Undersea .

ontologyofspatialobject:waterfall-s-
      a       owl:Class ;
      rdfs:comment "waterfall(s).  a perpendicular or very steep descent of the water of a stream"@en ;
      rdfs:subClassOf ontologyofspatialobject:Hydrographic .

ontologyofspatialobject:airbase
      a       owl:Class ;
      rdfs:comment "airbase.  an area used to store supplies, provide barracks for air force personnel, hangars and runways for aircraft, and from which operations are initiated"@en ;
      rdfs:subClassOf ontologyofspatialobject:Spot .

ontologyofspatialobject:oil-palm-plantation
      a       owl:Class ;
      rdfs:comment "oil palm plantation.  an estate specializing in the cultivation of oil palm trees"@en ;
      rdfs:subClassOf ontologyofspatialobject:Spot .

ontologyofspatialobject:administrative
      a       owl:Class ;
      rdfs:subClassOf ontologyofspatialobject:boundary .

ontologyofspatialobject:salt-area
      a       owl:Class ;
      rdfs:comment "salt area.  a shallow basin or flat where salt accumulates after periodic inundation"@en ;
      rdfs:subClassOf ontologyofspatialobject:Area .

ontologyofspatialobject:mosque
      a       owl:Class ;
      rdfs:comment "mosque.  a building for public Islamic worship"@en ;
      rdfs:subClassOf ontologyofspatialobject:Spot .

ontologyofspatialobject:tunnels
      a       owl:Class ;
      rdfs:comment "tunnels.  subterranean passageways for transportation"@en ;
      rdfs:subClassOf ontologyofspatialobject:Road .

ontologyofspatialobject:delta
      a       owl:Class ;
      rdfs:comment "delta.  a flat plain formed by alluvial deposits at the mouth of a stream"@en ;
      rdfs:subClassOf ontologyofspatialobject:Hypsographic .

ontologyofspatialobject:current
      a       owl:Class ;
      rdfs:comment "current.  a horizontal flow of water in a given direction with uniform velocity"@en ;
      rdfs:subClassOf ontologyofspatialobject:Hydrographic .

ontologyofspatialobject:stream-bank
      a       owl:Class ;
      rdfs:comment "stream bank.  a sloping margin of a stream channel which normally confines the stream to its channel on land"@en ;
      rdfs:subClassOf ontologyofspatialobject:Hydrographic .

ontologyofspatialobject:seamounts
      a       owl:Class ;
      rdfs:comment "seamounts.  elevations rising generally more than 1,000 meters and of limited extent across the summit"@en ;
      rdfs:subClassOf ontologyofspatialobject:Undersea .

ontologyofspatialobject:cirque
      a       owl:Class ;
      rdfs:comment "cirque.  a bowl-like hollow partially surrounded by cliffs or steep slopes at the head of a glaciated valley"@en ;
      rdfs:subClassOf ontologyofspatialobject:Hypsographic .

ontologyofspatialobject:PopulatedPlace
      a       owl:Class ;
      rdfs:comment "P city, village,..."@en ;
      rdfs:subClassOf ontologyofspatialobject:GeonameConcept , ontologyofspatialobject:place .

ontologyofspatialobject:reach
      a       owl:Class ;
      rdfs:comment "reach.  a straight section of a navigable stream or channel between two bends"@en ;
      rdfs:subClassOf ontologyofspatialobject:Hydrographic .

ontologyofspatialobject:talus-slope
      a       owl:Class ;
      rdfs:comment "talus slope.  a steep concave slope formed by an accumulation of loose rock fragments at the base of a cliff or steep slope"@en ;
      rdfs:subClassOf ontologyofspatialobject:Hypsographic .

[]    a       owl:AllDisjointProperties ;
      owl:members (ontologyofspatialobject:countryName ontologyofspatialobject:elevation ontologyofspatialobject:feature ontologyofspatialobject:featureClass ontologyofspatialobject:featureClassName ontologyofspatialobject:featureCodeName ontologyofspatialobject:language ontologyofspatialobject:name ontologyofspatialobject:rank ontologyofspatialobject:style ontologyofspatialobject:summary ontologyofspatialobject:taqs ontologyofspatialobject:thumbnailImg ontologyofspatialobject:timezone ontologyofspatialobject:title ontologyofspatialobject:type ontologyofspatialobject:typeRelation ontologyofspatialobject:wikipediaUrl ontologyofspatialobject:wkt) .

[]    a       owl:AllDisjointProperties ;
      owl:members (ontologyofspatialobject:adminCode1 ontologyofspatialobject:adminCode2 ontologyofspatialobject:adminCode3 ontologyofspatialobject:adminCode4 ontologyofspatialobject:adminCode5 ontologyofspatialobject:adminName1 ontologyofspatialobject:boundingBox ontologyofspatialobject:taqs ontologyofspatialobject:typeRelation ontologyofspatialobject:wikipediaUrl ontologyofspatialobject:wkt) .

ontologyofspatialobject:college
      a       owl:Class ;
      rdfs:comment "college.  the grounds and buildings of an institution of higher learning"@en ;
      rdfs:subClassOf ontologyofspatialobject:Spot .

ontologyofspatialobject:slope-s-
      a       owl:Class ;
      rdfs:comment "slope(s).  a surface with a relatively uniform slope angle"@en ;
      rdfs:subClassOf ontologyofspatialobject:Hypsographic .

ontologyofspatialobject:historical-region
      a       owl:Class ;
      rdfs:comment "historical region.  a former historic area distinguished by one or more observable physical or cultural characteristics"@en ;
      rdfs:subClassOf ontologyofspatialobject:Area .

ontologyofspatialobject:cleft-s-
      a       owl:Class ;
      rdfs:comment "cleft(s).  a deep narrow slot, notch, or groove in a coastal cliff"@en ;
      rdfs:subClassOf ontologyofspatialobject:Hypsographic .

ontologyofspatialobject:pan
      a       owl:Class ;
      rdfs:comment "pan.  a near-level shallow, natural depression or basin, usually containing an intermittent lake, pond, or pool"@en ;
      rdfs:subClassOf ontologyofspatialobject:Hypsographic .

ontologyofspatialobject:park-gate
      a       owl:Class ;
      rdfs:comment "park gate.  a controlled access to a park"@en ;
      rdfs:subClassOf ontologyofspatialobject:Spot .

ontologyofspatialobject:sound
      a       owl:Class ;
      rdfs:comment "sound.   or connecting two larger bodies of water\""@en ;
      rdfs:subClassOf ontologyofspatialobject:Hydrographic .

ontologyofspatialobject:lake-channel-s-
      a       owl:Class ;
      rdfs:comment "lake channel(s).  that part of a lake having water deep enough for navigation between islands, shoals, etc."@en ;
      rdfs:subClassOf ontologyofspatialobject:Hydrographic .

ontologyofspatialobject:historical-capital-of-a-political-entity
      a       owl:Class ;
      rdfs:comment "historical capital of a political entity.  a former capital of a political entity"@en ;
      rdfs:subClassOf ontologyofspatialobject:PopulatedPlace .

ontologyofspatialobject:salt-marsh
      a       owl:Class ;
      rdfs:comment "salt marsh.  a flat area, subject to periodic salt water inundation, dominated by grassy salt-tolerant plants"@en ;
      rdfs:subClassOf ontologyofspatialobject:Hydrographic .

ontologyofspatialobject:seat-of-a-fourth-order-administrative-division
      a       owl:Class ;
      rdfs:comment "seat of a fourth-order administrative division.  "@en ;
      rdfs:subClassOf ontologyofspatialobject:PopulatedPlace .

ontologyofspatialobject:Hypsographic
      a       owl:Class ;
      rdfs:comment "Hypsographic"@en ;
      rdfs:subClassOf ontologyofspatialobject:GeonameConcept , ontologyofspatialobject:natural .

ontologyofspatialobject:grazing-area
      a       owl:Class ;
      rdfs:comment "grazing area.  an area of grasses and shrubs used for grazing"@en ;
      rdfs:subClassOf ontologyofspatialobject:Area .

ontologyofspatialobject:university
      a       owl:Class ;
      rdfs:comment "university.  An institution for higher learning with teaching and research facilities constituting a graduate school and professional schools that award master's degrees and doctorates and an undergraduate division that awards bachelor's degrees."@en ;
      rdfs:subClassOf ontologyofspatialobject:Spot .

ontologyofspatialobject:isSouthOf
      a       owl:TransitiveProperty , owl:ObjectProperty ;
      rdfs:comment "is South of"@en ;
      rdfs:domain ontologyofspatialobject:SpatialObject ;
      rdfs:range ontologyofspatialobject:SpatialObject ;
      rdfs:subPropertyOf ontologyofspatialobject:directional .

ontologyofspatialobject:polder
      a       owl:Class ;
      rdfs:comment "polder.  an area reclaimed from the sea by diking and draining"@en ;
      rdfs:subClassOf ontologyofspatialobject:Hypsographic .

ontologyofspatialobject:sugar-mill
      a       owl:Class ;
      rdfs:comment "sugar mill.  a facility where sugar cane is processed into raw sugar"@en ;
      rdfs:subClassOf ontologyofspatialobject:Spot .

ontologyofspatialobject:intersects
      a       owl:ObjectProperty , owl:SymmetricProperty ;
      rdfs:comment """Two geometries intersect if they share at least one point in common. 

http://esri.github.io/geometry-api-java/doc/Intersects.html (There is a conceptual mistake in the url of ESRI, when they say: \"Intersects is the inverse of Disjoint\")"""@en ;
      rdfs:domain ontologyofspatialobject:SpatialObject ;
      rdfs:range ontologyofspatialobject:SpatialObject ;
      rdfs:subPropertyOf ontologyofspatialobject:topological .

ontologyofspatialobject:icecap
      a       owl:Class ;
      rdfs:comment "icecap.   smaller than an ice sheet\""@en ;
      rdfs:subClassOf ontologyofspatialobject:Hydrographic .

ontologyofspatialobject:first-order-administrative-division
      a       owl:Class ;
      rdfs:comment "first-order administrative division.  a primary administrative division of a country, such as a state in the United States"@en ;
      rdfs:subClassOf ontologyofspatialobject:AdministrativeBoundary .

ontologyofspatialobject:road-junction
      a       owl:Class ;
      rdfs:comment "road junction.  a place where two or more roads join"@en ;
      rdfs:subClassOf ontologyofspatialobject:Road .

ontologyofspatialobject:divide
      a       owl:Class ;
      rdfs:comment "divide.  a line separating adjacent drainage basins"@en ;
      rdfs:subClassOf ontologyofspatialobject:Hypsographic .

ontologyofspatialobject:region
      a       owl:Class ;
      rdfs:comment "region.  an area distinguished by one or more observable physical or cultural characteristics"@en ;
      rdfs:subClassOf ontologyofspatialobject:Area .

ontologyofspatialobject:lost-river
      a       owl:Class ;
      rdfs:comment "lost river.  a surface stream that disappears into an underground channel, or dries up in an arid area"@en ;
      rdfs:subClassOf ontologyofspatialobject:Hydrographic .

ontologyofspatialobject:business-center
      a       owl:Class ;
      rdfs:comment "business center.  a place where a number of businesses are located"@en ;
      rdfs:subClassOf ontologyofspatialobject:Area .

ontologyofspatialobject:historical-political-entity
      a       owl:Class ;
      rdfs:comment "historical political entity.  a former political entity"@en ;
      rdfs:subClassOf ontologyofspatialobject:AdministrativeBoundary .

ontologyofspatialobject:intermittent-pool
      a       owl:Class ;
      rdfs:comment "intermittent pool.  "@en ;
      rdfs:subClassOf ontologyofspatialobject:Hydrographic .

ontologyofspatialobject:hanging-valley
      a       owl:Class ;
      rdfs:comment "hanging valley.   most common in areas that have been glaciated\""@en ;
      rdfs:subClassOf ontologyofspatialobject:Hypsographic .

ontologyofspatialobject:bar
      a       owl:Class ;
      rdfs:comment "bar.  a shallow ridge or mound of coarse unconsolidated material in a stream channel, at the mouth of a stream, estuary, or lagoon and in the wave-break zone along coasts"@en ;
      rdfs:subClassOf ontologyofspatialobject:Hypsographic .

ontologyofspatialobject:Natural-watercourses
      a       owl:Class ;
      rdfs:subClassOf ontologyofspatialobject:Hydrographic .

ontologyofspatialobject:wikipediaDataProperty
      a       owl:FunctionalProperty , owl:DatatypeProperty ;
      rdfs:domain ontologyofspatialobject:SpatialObject ;
      rdfs:range rdfs:Literal .

ontologyofspatialobject:police-post
      a       owl:Class ;
      rdfs:comment "police post.  a building in which police are stationed"@en ;
      rdfs:subClassOf ontologyofspatialobject:Spot .

ontologyofspatialobject:restaurant
      a       owl:Class ;
      rdfs:comment "restaurant.  A place where meals are served to the public"@en ;
      rdfs:subClassOf ontologyofspatialobject:Spot .

ontologyofspatialobject:oil-refinery
      a       owl:Class ;
      rdfs:comment "oil refinery.  a facility for converting crude oil into refined petroleum products"@en ;
      rdfs:subClassOf ontologyofspatialobject:Spot .

ontologyofspatialobject:political-entity
      a       owl:Class ;
      rdfs:comment "political entity.  "@en ;
      rdfs:subClassOf ontologyofspatialobject:AdministrativeBoundary .

ontologyofspatialobject:industrial-area
      a       owl:Class ;
      rdfs:comment "industrial area.  an area characterized by industrial activity"@en ;
      rdfs:subClassOf ontologyofspatialobject:Area .

ontologyofspatialobject:salt-evaporation-ponds
      a       owl:Class ;
      rdfs:comment "salt evaporation ponds.  diked salt ponds used in the production of solar evaporated salt"@en ;
      rdfs:subClassOf ontologyofspatialobject:Hydrographic .

ontologyofspatialobject:ruin-s-
      a       owl:Class ;
      rdfs:comment "ruin(s).  a destroyed or decayed structure which is no longer functional"@en ;
      rdfs:subClassOf ontologyofspatialobject:Spot .

ontologyofspatialobject:hotel
      a       owl:Class ;
      rdfs:comment "hotel.  a building providing lodging and/or meals for the public"@en ;
      rdfs:subClassOf ontologyofspatialobject:Spot .

ontologyofspatialobject:seaplane-landing-area
      a       owl:Class ;
      rdfs:comment "seaplane landing area.  a place on a waterbody where floatplanes land and take off"@en ;
      rdfs:subClassOf ontologyofspatialobject:Man-made-waterways , ontologyofspatialobject:Hydrographic .

ontologyofspatialobject:Road
      a       owl:Class ;
      rdfs:comment "R road, railroad"@en ;
      rdfs:subClassOf ontologyofspatialobject:GeonameConcept , ontologyofspatialobject:landmark .

ontologyofspatialobject:overlap
      a       owl:ObjectProperty , owl:SymmetricProperty ;
      rdfs:comment """Two geometries overlap if they have the same dimension, and their intersection also has the same dimension but is different from both of them. 

Superposicion

http://esri.github.io/geometry-api-java/doc/Overlaps.html"""@es ;
      rdfs:domain ontologyofspatialobject:SpatialObject ;
      rdfs:range ontologyofspatialobject:SpatialObject ;
      rdfs:subPropertyOf ontologyofspatialobject:topological .

ontologyofspatialobject:tank-farm
      a       owl:Class ;
      rdfs:comment "tank farm.  a tract of land occupied by large, cylindrical, metal tanks in which oil or liquid petrochemicals are stored"@en ;
      rdfs:subClassOf ontologyofspatialobject:Spot .

ontologyofspatialobject:province
      a       owl:Class ;
      rdfs:comment "province.  a region identifiable by a group of similar physiographic features whose characteristics are markedly in contrast with surrounding areas"@en ;
      rdfs:subClassOf ontologyofspatialobject:Undersea .

ontologyofspatialobject:monument
      a       owl:Class ;
      rdfs:comment "monument.  a commemorative structure or statue"@en ;
      rdfs:subClassOf ontologyofspatialobject:Spot .

ontologyofspatialobject:reformatory
      a       owl:Class ;
      rdfs:comment "reformatory.  a facility for confining, training, and reforming young law offenders"@en ;
      rdfs:subClassOf ontologyofspatialobject:Spot .

ontologyofspatialobject:glacier-s-
      a       owl:Class ;
      rdfs:comment "glacier(s).  a mass of ice, usually at high latitudes or high elevations, with sufficient thickness to flow away from the source area in lobes, tongues, or masses"@en ;
      rdfs:subClassOf ontologyofspatialobject:Water , ontologyofspatialobject:Hydrographic .

ontologyofspatialobject:halting-place
      a       owl:Class ;
      rdfs:comment "halting place.  a place where caravans stop for rest"@en ;
      rdfs:subClassOf ontologyofspatialobject:Spot .

ontologyofspatialobject:headwaters
      a       owl:Class ;
      rdfs:comment "headwaters.  the source and upper part of a stream, including the upper drainage basin"@en ;
      rdfs:subClassOf ontologyofspatialobject:Hydrographic .

ontologyofspatialobject:oxbow-lake
      a       owl:Class ;
      rdfs:comment "oxbow lake.  a crescent-shaped lake commonly found adjacent to meandering streams"@en ;
      rdfs:subClassOf ontologyofspatialobject:Hydrographic .

ontologyofspatialobject:Continent
      a       owl:Class ;
      rdfs:comment "Continents"@en ;
      rdfs:subClassOf ontologyofspatialobject:AdministrativeBoundary .

ontologyofspatialobject:salt-mine-s-
      a       owl:Class ;
      rdfs:comment "salt mine(s).  a mine from which salt is extracted"@en ;
      rdfs:subClassOf ontologyofspatialobject:Spot .

ontologyofspatialobject:bay
      a       owl:Class ;
      rdfs:comment "bay.  a coastal indentation between two capes or headlands, larger than a cove but smaller than a gulf"@en ;
      rdfs:subClassOf ontologyofspatialobject:Natural-watercourses , ontologyofspatialobject:Hydrographic .

ontologyofspatialobject:cape
      a       owl:Class ;
      rdfs:comment "cape.  a land area, more prominent than a point, projecting into the sea and marking a notable change in coastal direction"@en ;
      rdfs:subClassOf ontologyofspatialobject:Hypsographic .

ontologyofspatialobject:section-of-stream
      a       owl:Class ;
      rdfs:comment "section of stream.  "@en ;
      rdfs:subClassOf ontologyofspatialobject:Hydrographic .

ontologyofspatialobject:spa
      a       owl:Class ;
      rdfs:comment "spa.  a resort area usually developed around a medicinal spring"@en ;
      rdfs:subClassOf ontologyofspatialobject:Spot .

ontologyofspatialobject:alternateNames
      a       owl:DatatypeProperty ;
      rdfs:comment """Stores the alternate names of place names in Geonames and OSM data

Sera utilizado tambien por OSM"""@en ;
      rdfs:domain ontologyofspatialobject:SpatialObject ;
      rdfs:range xsd:string ;
      rdfs:subPropertyOf ontologyofspatialobject:gonameDataProperty .

ontologyofspatialobject:navigation-channel
      a       owl:Class ;
      rdfs:comment "navigation channel.  a buoyed channel of sufficient depth for the safe navigation of vessels"@en ;
      rdfs:subClassOf ontologyofspatialobject:Hydrographic .

ontologyofspatialobject:gulf
      a       owl:Class ;
      rdfs:comment "gulf.  a large recess in the coastline, larger than a bay"@en ;
      rdfs:subClassOf ontologyofspatialobject:Hydrographic .

ontologyofspatialobject:beach-ridge
      a       owl:Class ;
      rdfs:comment "beach ridge.  a ridge of sand just inland and parallel to the beach, usually in series"@en ;
      rdfs:subClassOf ontologyofspatialobject:Hypsographic .

ontologyofspatialobject:iron-mine-s-
      a       owl:Class ;
      rdfs:comment "iron mine(s).  a mine where iron ore is extracted"@en ;
      rdfs:subClassOf ontologyofspatialobject:Spot .

ontologyofspatialobject:united-states-government-establishment
      a       owl:Class ;
      rdfs:comment "united states government establishment.  a facility operated by the United States Government in Panama"@en ;
      rdfs:subClassOf ontologyofspatialobject:Spot .

ontologyofspatialobject:canal
      a       owl:Class ;
      rdfs:comment "canal.  an artificial watercourse"@en ;
      rdfs:subClassOf ontologyofspatialobject:Man-made-waterways , ontologyofspatialobject:Hydrographic .

ontologyofspatialobject:olive-grove
      a       owl:Class ;
      rdfs:comment "olive grove.  a planting of olive trees"@en ;
      rdfs:subClassOf ontologyofspatialobject:Vegetation .

ontologyofspatialobject:mountains
      a       owl:Class ;
      rdfs:comment "mountains.  a mountain range or a group of mountains or high ridges"@en ;
      rdfs:subClassOf ontologyofspatialobject:Hypsographic .

ontologyofspatialobject:countryName
      a       owl:FunctionalProperty , owl:DatatypeProperty ;
      rdfs:comment "countryName"@en ;
      rdfs:domain ontologyofspatialobject:SpatialObject ;
      rdfs:range xsd:string ;
      rdfs:subPropertyOf ontologyofspatialobject:gonameDataProperty .

ontologyofspatialobject:homestead
      a       owl:Class ;
      rdfs:comment "homestead.  a residence, owner's or manager's, on a sheep or cattle station, woolshed, outcamp, or Aboriginal outstation, specific to Australia and New Zealand"@en ;
      rdfs:subClassOf ontologyofspatialobject:Spot .

ontologyofspatialobject:forest-s-
      a       owl:Class ;
      rdfs:comment "forest(s).  an area dominated by tree vegetation"@en ;
      rdfs:subClassOf ontologyofspatialobject:Vegetation .

ontologyofspatialobject:sandy-desert
      a       owl:Class ;
      rdfs:comment "sandy desert.  an extensive tract of shifting sand and sand dunes"@en ;
      rdfs:subClassOf ontologyofspatialobject:Hypsographic .

ontologyofspatialobject:copper-mine-s-
      a       owl:Class ;
      rdfs:comment "copper mine(s).  a mine where copper ore is extracted"@en ;
      rdfs:subClassOf ontologyofspatialobject:Spot .

ontologyofspatialobject:transit-terminal
      a       owl:Class ;
      rdfs:comment "transit terminal.  facilities for the handling of vehicular freight and passengers"@en ;
      rdfs:subClassOf ontologyofspatialobject:Spot .

ontologyofspatialobject:area
      a       owl:Class ;
      rdfs:comment "area.  a tract of land without homogeneous character or boundaries"@en ;
      rdfs:subClassOf ontologyofspatialobject:Area .

ontologyofspatialobject:mound-s-
      a       owl:Class ;
      rdfs:comment "mound(s).  a low, isolated, rounded hill"@en ;
      rdfs:subClassOf ontologyofspatialobject:Hypsographic .

ontologyofspatialobject:reserve
      a       owl:Class ;
      rdfs:comment "reserve.  a tract of public land reserved for future use or restricted as to use"@en ;
      rdfs:subClassOf ontologyofspatialobject:Area .

ontologyofspatialobject:administrative-division
      a       owl:Class ;
      rdfs:comment "administrative division.  an administrative division of a country, undifferentiated as to administrative level"@en ;
      rdfs:subClassOf ontologyofspatialobject:AdministrativeBoundary .

ontologyofspatialobject:fort
      a       owl:Class ;
      rdfs:comment "fort.  a defensive structure or earthworks"@en ;
      rdfs:subClassOf ontologyofspatialobject:Spot .

ontologyofspatialobject:maritime-school
      a       owl:Class ;
      rdfs:comment "maritime school.  a school at which maritime sciences form the core of the curriculum"@en ;
      rdfs:subClassOf ontologyofspatialobject:Spot .

ontologyofspatialobject:inlet
      a       owl:Class ;
      rdfs:comment "inlet.  a narrow waterway extending into the land, or connecting a bay or lagoon with a larger body of water"@en ;
      rdfs:subClassOf ontologyofspatialobject:Hydrographic .

ontologyofspatialobject:farms
      a       owl:Class ;
      rdfs:comment "farms.  tracts of land with associated buildings devoted to agriculture"@en ;
      rdfs:subClassOf ontologyofspatialobject:Spot .

ontologyofspatialobject:reef
      a       owl:Class ;
      rdfs:comment "reef.  a surface-navigation hazard composed of consolidated material"@en ;
      rdfs:subClassOf ontologyofspatialobject:Undersea .

ontologyofspatialobject:natural-tunnel
      a       owl:Class ;
      rdfs:comment "natural tunnel.  a cave that is open at both ends"@en ;
      rdfs:subClassOf ontologyofspatialobject:Road .

ontologyofspatialobject:bridge
      a       owl:Class ;
      rdfs:comment "bridge.  a structure erected across an obstacle such as a stream, road, etc., in order to carry roads, railroads, and pedestrians across"@en ;
      rdfs:subClassOf ontologyofspatialobject:Spot .

ontologyofspatialobject:thumbnailImg
      a       owl:DatatypeProperty ;
      rdfs:comment "URL of a small thumbnail image"@en ;
      rdfs:domain ontologyofspatialobject:SpatialObject ;
      rdfs:range xsd:string ;
      rdfs:subPropertyOf ontologyofspatialobject:wikipediaDataProperty .

ontologyofspatialobject:heath
      a       owl:Class ;
      rdfs:comment "heath.  an upland moor or sandy area dominated by low shrubby vegetation including heather"@en ;
      rdfs:subClassOf ontologyofspatialobject:Vegetation .

ontologyofspatialobject:intermittent-wetland
      a       owl:Class ;
      rdfs:comment "intermittent wetland.  "@en ;
      rdfs:subClassOf ontologyofspatialobject:Hydrographic .

ontologyofspatialobject:bays
      a       owl:Class ;
      rdfs:comment "bays.  coastal indentations between two capes or headlands, larger than a cove but smaller than a gulf"@en ;
      rdfs:subClassOf ontologyofspatialobject:Natural-watercourses , ontologyofspatialobject:Hydrographic .

ontologyofspatialobject:territory
      a       owl:Class ;
      rdfs:comment "territory.  "@en ;
      rdfs:subClassOf ontologyofspatialobject:AdministrativeBoundary .

ontologyofspatialobject:headland
      a       owl:Class ;
      rdfs:comment "headland.  a high projection of land extending into a large body of water beyond the line of the coast"@en ;
      rdfs:subClassOf ontologyofspatialobject:Hypsographic .

ontologyofspatialobject:gonameDataProperty
      a       owl:DatatypeProperty ;
      rdfs:comment "Encapsulates the data properties Geonames"@en ;
      rdfs:domain ontologyofspatialobject:SpatialObject ;
      rdfs:range rdfs:Literal .

ontologyofspatialobject:stream
      a       owl:Class ;
      rdfs:comment "stream.  a body of running water moving to a lower level in a channel on land"@en ;
      rdfs:subClassOf ontologyofspatialobject:Hydrographic .

ontologyofspatialobject:tribal-area
      a       owl:Class ;
      rdfs:comment "tribal area.  a tract of land used by nomadic or other tribes"@en ;
      rdfs:subClassOf ontologyofspatialobject:Area .

ontologyofspatialobject:leprosarium
      a       owl:Class ;
      rdfs:comment "leprosarium.  an asylum or hospital for lepers"@en ;
      rdfs:subClassOf ontologyofspatialobject:Spot .

ontologyofspatialobject:vineyards
      a       owl:Class ;
      rdfs:comment "vineyards.  plantings of grapevines"@en ;
      rdfs:subClassOf ontologyofspatialobject:Vegetation .

ontologyofspatialobject:dike
      a       owl:Class ;
      rdfs:comment "dike.  an earth or stone embankment usually constructed for flood or stream control"@en ;
      rdfs:subClassOf ontologyofspatialobject:Spot .

ontologyofspatialobject:historical-second-order-administrative-division
      a       owl:Class ;
      rdfs:comment "historical second-order administrative division.  a former second-order administrative division"@en ;
      rdfs:subClassOf ontologyofspatialobject:AdministrativeBoundary .

ontologyofspatialobject:wkt
      a       owl:FunctionalProperty , owl:DatatypeProperty ;
      rdfs:comment "Representa la cadena WKT de los objetos. Se utiliza por todas las fuentes de datos."@es ;
      rdfs:domain ontologyofspatialobject:SpatialObject ;
      rdfs:range xsd:string ;
      rdfs:subPropertyOf owl:topDataProperty .

ontologyofspatialobject:former-sugar-mill
      a       owl:Class ;
      rdfs:comment "former sugar mill.  a sugar mill no longer used as a sugar mill"@en ;
      rdfs:subClassOf ontologyofspatialobject:Spot .

ontologyofspatialobject:whirlpool
      a       owl:Class ;
      rdfs:comment "whirlpool.  a turbulent, rotating movement of water in a stream"@en ;
      rdfs:subClassOf ontologyofspatialobject:Hydrographic .

ontologyofspatialobject:buffer-zone
      a       owl:Class ;
      rdfs:comment "buffer zone.  a zone recognized as a buffer between two nations in which military presence is minimal or absent"@en ;
      rdfs:subClassOf ontologyofspatialobject:AdministrativeBoundary .

ontologyofspatialobject:port
      a       owl:Class ;
      rdfs:comment "port.  a place provided with terminal and transfer facilities for loading and discharging waterborne cargo or passengers, usually located in a harbor"@en ;
      rdfs:subClassOf ontologyofspatialobject:Area .

ontologyofspatialobject:ditch
      a       owl:Class ;
      rdfs:comment "ditch.  a small artificial watercourse dug for draining or irrigating the land"@en ;
      rdfs:subClassOf ontologyofspatialobject:Man-made-waterways , ontologyofspatialobject:Hydrographic .

ontologyofspatialobject:monastery
      a       owl:Class ;
      rdfs:comment "monastery.  a building and grounds where a community of monks lives in seclusion"@en ;
      rdfs:subClassOf ontologyofspatialobject:Spot .

ontologyofspatialobject:dune-s-
      a       owl:Class ;
      rdfs:comment "dune(s).  a wave form, ridge or star shape feature composed of sand"@en ;
      rdfs:subClassOf ontologyofspatialobject:Hypsographic .

ontologyofspatialobject:shoal
      a       owl:Class ;
      rdfs:comment "shoal.  a surface-navigation hazard composed of unconsolidated material"@en ;
      rdfs:subClassOf ontologyofspatialobject:Undersea .

ontologyofspatialobject:sport
      a       owl:Class ;
      rdfs:comment "This is used to provide information about which sports are placed on a facility such as a pitch or stadium. See the page titled Sport(\"http://wiki.openstreetmap.org/wiki/Sport\") for an introduction on its usage."@en ;
      rdfs:subClassOf ontologyofspatialobject:SpatialObject .

ontologyofspatialobject:landing
      a       owl:Class ;
      rdfs:comment "landing.  a place where boats receive or discharge passengers and freight, but lacking most port facilities"@en ;
      rdfs:subClassOf ontologyofspatialobject:Spot .

ontologyofspatialobject:slope
      a       owl:Class ;
      rdfs:comment "slope.  the slope seaward from the shelf edge to the beginning of a continental rise or the point where there is a general reduction in slope"@en ;
      rdfs:subClassOf ontologyofspatialobject:Undersea .

ontologyofspatialobject:lock-s-
      a       owl:Class ;
      rdfs:comment "lock(s).  a basin in a waterway with gates at each end by means of which vessels are passed from one water level to another"@en ;
      rdfs:subClassOf ontologyofspatialobject:Spot .

ontologyofspatialobject:tidal-creek-s-
      a       owl:Class ;
      rdfs:comment "tidal creek(s).  a meandering channel in a coastal wetland subject to bi-directional tidal currents"@en ;
      rdfs:subClassOf ontologyofspatialobject:Hydrographic .

ontologyofspatialobject:intermittent-lake
      a       owl:Class ;
      rdfs:comment "intermittent lake.  "@en ;
      rdfs:subClassOf ontologyofspatialobject:Hydrographic .

ontologyofspatialobject:peak
      a       owl:Class ;
      rdfs:comment "peak.  a prominent elevation, part of a larger feature, either pointed or of very limited extent across the summit"@en , "peak.  a pointed elevation atop a mountain, ridge, or other hypsographic feature"@en ;
      rdfs:subClassOf ontologyofspatialobject:Hypsographic , ontologyofspatialobject:Undersea .

ontologyofspatialobject:NortHemisphere
      a       owl:Class ;
      rdfs:comment "North Hemisphere"@en ;
      rdfs:subClassOf ontologyofspatialobject:AdministrativeBoundary ;
      owl:disjointWith ontologyofspatialobject:SurtHemisphere .

ontologyofspatialobject:sinkhole
      a       owl:Class ;
      rdfs:comment "sinkhole.  a small crater-shape depression in a karst area"@en ;
      rdfs:subClassOf ontologyofspatialobject:Hypsographic .

ontologyofspatialobject:canyons
      a       owl:Class ;
      rdfs:comment "canyons.  relatively narrow, deep depressions with steep sides, the bottom of which generally has a continuous slope"@en ;
      rdfs:subClassOf ontologyofspatialobject:Undersea .

ontologyofspatialobject:portage
      a       owl:Class ;
      rdfs:comment "portage.  a place where boats, goods, etc., are carried overland between navigable waters"@en ;
      rdfs:subClassOf ontologyofspatialobject:Road .

ontologyofspatialobject:city
      a       owl:Class ;
      rdfs:subClassOf ontologyofspatialobject:PopulatedPlace .

ontologyofspatialobject:state
      a       owl:Class ;
      rdfs:subClassOf ontologyofspatialobject:place .

ontologyofspatialobject:automatic-teller-machine
      a       owl:Class ;
      rdfs:comment "automatic teller machine.  An unattended electronic machine in a public place, connected to a data system and related equipment and activated by a bank customer to obtain cash withdrawals and other banking services."@en ;
      rdfs:subClassOf ontologyofspatialobject:Spot .

ontologyofspatialobject:sheepfold
      a       owl:Class ;
      rdfs:comment "sheepfold.  a fence or wall enclosure for sheep and other small herd animals"@en ;
      rdfs:subClassOf ontologyofspatialobject:Spot .

ontologyofspatialobject:valley
      a       owl:Class ;
      rdfs:comment "valley.  a relatively shallow, wide depression, the bottom of which usually has a continuous gradient"@en , "valley.  an elongated depression usually traversed by a stream"@en ;
      rdfs:subClassOf ontologyofspatialobject:Hypsographic , ontologyofspatialobject:Undersea .

ontologyofspatialobject:seat-of-a-first-order-administrative-division
      a       owl:Class ;
      rdfs:comment "seat of a first-order administrative division.  seat of a first-order administrative division (PPLC takes precedence over PPLA)"@en ;
      rdfs:subClassOf ontologyofspatialobject:PopulatedPlace .

ontologyofspatialobject:marsh-es-
      a       owl:Class ;
      rdfs:comment "marsh(es).  a wetland dominated by grass-like vegetation"@en ;
      rdfs:subClassOf ontologyofspatialobject:Hydrographic .

ontologyofspatialobject:points
      a       owl:Class ;
      rdfs:comment "points.  tapering pieces of land projecting into a body of water, less prominent than a cape"@en ;
      rdfs:subClassOf ontologyofspatialobject:Hypsographic .

ontologyofspatialobject:military-base
      a       owl:Class ;
      rdfs:comment "military base.  a place used by an army or other armed service for storing arms and supplies, and for accommodating and training troops, a base from which operations can be initiated"@en ;
      rdfs:subClassOf ontologyofspatialobject:Area .

ontologyofspatialobject:cannery
      a       owl:Class ;
      rdfs:comment "cannery.  a building where food items are canned"@en ;
      rdfs:subClassOf ontologyofspatialobject:Spot .

<urn:swrl#latitudy>
      a       swrl:Variable .

ontologyofspatialobject:abandoned-mine
      a       owl:Class ;
      rdfs:comment "abandoned mine.  "@en ;
      rdfs:subClassOf ontologyofspatialobject:Spot .

ontologyofspatialobject:causeway
      a       owl:Class ;
      rdfs:comment "causeway.  a raised roadway across wet ground or shallow water"@en ;
      rdfs:subClassOf ontologyofspatialobject:Road .

ontologyofspatialobject:longitude
      a       owl:FunctionalProperty , owl:DatatypeProperty ;
      rdfs:comment "Es utilizada por Geonames, OSM y por Wikipedia" ;
      rdfs:domain ontologyofspatialobject:SpatialObject ;
      rdfs:range xsd:double ;
      rdfs:subPropertyOf owl:topDataProperty .

ontologyofspatialobject:SurtHemisphere
      a       owl:Class ;
      rdfs:comment "Surt Hemisphere"@en ;
      rdfs:subClassOf ontologyofspatialobject:AdministrativeBoundary .

ontologyofspatialobject:field-s-
      a       owl:Class ;
      rdfs:comment "field(s).  an open as opposed to wooded area"@en ;
      rdfs:subClassOf ontologyofspatialobject:Area .

ontologyofspatialobject:adminName2
      a       owl:FunctionalProperty , owl:DatatypeProperty ;
      rdfs:comment "adminName2"@en ;
      rdfs:domain ontologyofspatialobject:SpatialObject ;
      rdfs:range xsd:string ;
      rdfs:subPropertyOf ontologyofspatialobject:gonameDataProperty .

ontologyofspatialobject:cliff-s-
      a       owl:Class ;
      rdfs:comment "cliff(s).  a high, steep to perpendicular slope overlooking a waterbody or lower area"@en ;
      rdfs:subClassOf ontologyofspatialobject:Hypsographic .

ontologyofspatialobject:cutoff
      a       owl:Class ;
      rdfs:comment "cutoff.  a channel formed as a result of a stream cutting through a meander neck"@en ;
      rdfs:subClassOf ontologyofspatialobject:Hydrographic .

ontologyofspatialobject:pier
      a       owl:Class ;
      rdfs:comment "pier.  a structure built out into navigable water on piles providing berthing for ships and recreation"@en ;
      rdfs:subClassOf ontologyofspatialobject:Spot .

ontologyofspatialobject:shore
      a       owl:Class ;
      rdfs:comment "shore.  a narrow zone bordering a waterbody which covers and uncovers at high and low water, respectively"@en ;
      rdfs:subClassOf ontologyofspatialobject:Hypsographic .

ontologyofspatialobject:fracture-zone
      a       owl:Class ;
      rdfs:comment "fracture zone.  an extensive linear zone of irregular topography of the sea floor, characterized by steep-sided or asymmetrical ridges, troughs, or escarpments"@en ;
      rdfs:subClassOf ontologyofspatialobject:Undersea .

ontologyofspatialobject:railroad-yard
      a       owl:Class ;
      rdfs:comment "railroad yard.  a system of tracks used for the making up of trains, and switching and storing freight cars"@en ;
      rdfs:subClassOf ontologyofspatialobject:Road .

ontologyofspatialobject:irrigated-field-s-
      a       owl:Class ;
      rdfs:comment "irrigated field(s).  a tract of level or terraced land which is irrigated"@en ;
      rdfs:subClassOf ontologyofspatialobject:Area .

ontologyofspatialobject:irrigation-ditch
      a       owl:Class ;
      rdfs:comment "irrigation ditch.  a ditch which serves to distribute irrigation water"@en ;
      rdfs:subClassOf ontologyofspatialobject:Man-made-waterways , ontologyofspatialobject:Hydrographic .

ontologyofspatialobject:satellite-station
      a       owl:Class ;
      rdfs:comment "satellite station.  a facility for tracking and communicating with orbiting satellites"@en ;
      rdfs:subClassOf ontologyofspatialobject:Spot .

terms:license
      a       owl:AnnotationProperty .

ontologyofspatialobject:continent
      a       owl:Class ;
      rdfs:comment "continent.  continent: Europe, Africa, Asia, North America, South America, Oceania, Antarctica"@en ;
      rdfs:subClassOf ontologyofspatialobject:Area .

ontologyofspatialobject:leased-area
      a       owl:Class ;
      rdfs:comment "leased area.  a tract of land leased to another country, usually for military installations"@en ;
      rdfs:subClassOf ontologyofspatialobject:AdministrativeBoundary .

ontologyofspatialobject:university-prep-school
      a       owl:Class ;
      rdfs:comment "university prep school.  University Preparation Schools & Institutions"@en ;
      rdfs:subClassOf ontologyofspatialobject:Spot .

ontologyofspatialobject:artillery-range
      a       owl:Class ;
      rdfs:comment "artillery range.  a tract of land used for artillery firing practice"@en ;
      rdfs:subClassOf ontologyofspatialobject:Area .

ontologyofspatialobject:adminName3
      a       owl:FunctionalProperty , owl:DatatypeProperty ;
      rdfs:comment "adminName3"@en ;
      rdfs:domain ontologyofspatialobject:SpatialObject ;
      rdfs:range xsd:string ;
      rdfs:subPropertyOf ontologyofspatialobject:gonameDataProperty .

ontologyofspatialobject:moat
      a       owl:Class ;
      rdfs:comment "moat.  an annular depression that may not be continuous, located at the base of many seamounts, islands, and other isolated elevations"@en ;
      rdfs:subClassOf ontologyofspatialobject:Undersea .

ontologyofspatialobject:huts
      a       owl:Class ;
      rdfs:comment "huts.  small primitive houses"@en ;
      rdfs:subClassOf ontologyofspatialobject:Spot .

ontologyofspatialobject:taqs
      a       owl:DatatypeProperty ;
      rdfs:comment "Es un par  formado de la siguiente forma: \"TaqsKey,TaqsValue\". Si tiene varios taqs, como casi siempre, se repitira este dataproperty em el individuo, es decir, este no es funcional."@es ;
      rdfs:domain ontologyofspatialobject:SpatialObject ;
      rdfs:range xsd:string ;
      rdfs:subPropertyOf ontologyofspatialobject:osmDataProperty .

ontologyofspatialobject:guest-house
      a       owl:Class ;
      rdfs:comment "guest house.  a house used to provide lodging for paying guests"@en ;
      rdfs:subClassOf ontologyofspatialobject:Spot .

ontologyofspatialobject:adminName4
      a       owl:FunctionalProperty , owl:DatatypeProperty ;
      rdfs:comment "adminName4"@en ;
      rdfs:domain ontologyofspatialobject:SpatialObject ;
      rdfs:range xsd:string ;
      rdfs:subPropertyOf ontologyofspatialobject:gonameDataProperty .

ontologyofspatialobject:observatory
      a       owl:Class ;
      rdfs:comment "observatory.  a facility equipped for observation of atmospheric or space phenomena"@en ;
      rdfs:subClassOf ontologyofspatialobject:Spot .

ontologyofspatialobject:mesa-s-
      a       owl:Class ;
      rdfs:comment "mesa(s).  a flat-topped, isolated elevation with steep slopes on all sides, less extensive than a plateau"@en ;
      rdfs:subClassOf ontologyofspatialobject:Hypsographic .

ontologyofspatialobject:abandoned-police-post
      a       owl:Class ;
      rdfs:comment "abandoned police post.  "@en ;
      rdfs:subClassOf ontologyofspatialobject:Spot .

ontologyofspatialobject:wildlife-reserve
      a       owl:Class ;
      rdfs:comment "wildlife reserve.  a tract of public land reserved for the preservation of wildlife"@en ;
      rdfs:subClassOf ontologyofspatialobject:Area .

ontologyofspatialobject:camp-s-
      a       owl:Class ;
      rdfs:comment "camp(s).  a site occupied by tents, huts, or other shelters for temporary use"@en ;
      rdfs:subClassOf ontologyofspatialobject:Spot .

ontologyofspatialobject:overfalls
      a       owl:Class ;
      rdfs:comment "overfalls.  an area of breaking waves caused by the meeting of currents or by waves moving against the current"@en ;
      rdfs:subClassOf ontologyofspatialobject:Hydrographic .

ontologyofspatialobject:sluice
      a       owl:Class ;
      rdfs:comment "sluice.  a conduit or passage for carrying off surplus water from a waterbody, usually regulated by means of a sluice gate"@en ;
      rdfs:subClassOf ontologyofspatialobject:Spot .

ontologyofspatialobject:ranch-es-
      a       owl:Class ;
      rdfs:comment "ranch(es).  a large farm specializing in extensive grazing of livestock"@en ;
      rdfs:subClassOf ontologyofspatialobject:Spot .

ontologyofspatialobject:labor-camp
      a       owl:Class ;
      rdfs:comment "labor camp.  a camp used by migrant or temporary laborers"@en ;
      rdfs:subClassOf ontologyofspatialobject:Spot .

ontologyofspatialobject:village
      a       owl:Class ;
      rdfs:subClassOf ontologyofspatialobject:place .

ontologyofspatialobject:astronomical-station
      a       owl:Class ;
      rdfs:comment "astronomical station.  a point on the earth whose position has been determined by observations of celestial bodies"@en ;
      rdfs:subClassOf ontologyofspatialobject:Spot .

ontologyofspatialobject:blowout-s-
      a       owl:Class ;
      rdfs:comment "blowout(s).  a small depression in sandy terrain, caused by wind erosion"@en ;
      rdfs:subClassOf ontologyofspatialobject:Hypsographic .

ontologyofspatialobject:adminName5
      a       owl:FunctionalProperty , owl:DatatypeProperty ;
      rdfs:comment "adminName5"@en ;
      rdfs:domain ontologyofspatialobject:SpatialObject ;
      rdfs:range xsd:string ;
      rdfs:subPropertyOf ontologyofspatialobject:gonameDataProperty .

ontologyofspatialobject:wikipediaUrl
      a       owl:DatatypeProperty ;
      rdfs:comment "URL of the article"@en ;
      rdfs:domain ontologyofspatialobject:SpatialObject ;
      rdfs:range xsd:string ;
      rdfs:subPropertyOf ontologyofspatialobject:wikipediaDataProperty .

ontologyofspatialobject:strait
      a       owl:Class ;
      rdfs:comment "strait.  a relatively narrow waterway, usually narrower and less extensive than a sound, connecting two larger bodies of water"@en ;
      rdfs:subClassOf ontologyofspatialobject:Hydrographic .

ontologyofspatialobject:temp-work-office
      a       owl:Class ;
      rdfs:comment "temp work office.  Temporary Work Offices"@en ;
      rdfs:subClassOf ontologyofspatialobject:Spot .

ontologyofspatialobject:hospital
      a       owl:Class ;
      rdfs:comment "hospital.  a building in which sick or injured, especially those confined to bed, are medically treated"@en ;
      rdfs:subClassOf ontologyofspatialobject:Spot .

ontologyofspatialobject:gravel-area
      a       owl:Class ;
      rdfs:comment "gravel area.  an area covered with gravel"@en ;
      rdfs:subClassOf ontologyofspatialobject:Area .

ontologyofspatialobject:orchard-s-
      a       owl:Class ;
      rdfs:comment "orchard(s).  a planting of fruit or nut trees"@en ;
      rdfs:subClassOf ontologyofspatialobject:Vegetation .

ontologyofspatialobject:farm
      a       owl:Class ;
      rdfs:comment "farm.  a tract of land with associated buildings devoted to agriculture"@en ;
      rdfs:subClassOf ontologyofspatialobject:Spot .

ontologyofspatialobject:mangrove-island
      a       owl:Class ;
      rdfs:comment "mangrove island.  a mangrove swamp surrounded by a waterbody"@en ;
      rdfs:subClassOf ontologyofspatialobject:Hypsographic .

ontologyofspatialobject:oil-camp
      a       owl:Class ;
      rdfs:comment "oil camp.  a camp used by oilfield workers"@en ;
      rdfs:subClassOf ontologyofspatialobject:Spot .

ontologyofspatialobject:historical-populated-place
      a       owl:Class ;
      rdfs:comment "historical populated place.  a populated place that no longer exists"@en ;
      rdfs:subClassOf ontologyofspatialobject:PopulatedPlace .

ontologyofspatialobject:railroad-signal
      a       owl:Class ;
      rdfs:comment "railroad signal.  a signal at the entrance of a particular section of track governing the movement of trains"@en ;
      rdfs:subClassOf ontologyofspatialobject:Spot .

ontologyofspatialobject:communication-center
      a       owl:Class ;
      rdfs:comment "communication center.  a facility, including buildings, antennae, towers and electronic equipment for receiving and transmitting information"@en ;
      rdfs:subClassOf ontologyofspatialobject:Spot .

ontologyofspatialobject:featureCodeName
      a       owl:FunctionalProperty , owl:DatatypeProperty ;
      rdfs:comment "featureCodeName"@en ;
      rdfs:domain ontologyofspatialobject:SpatialObject ;
      rdfs:range xsd:string ;
      rdfs:subPropertyOf ontologyofspatialobject:gonameDataProperty .

ontologyofspatialobject:clinic
      a       owl:Class ;
      rdfs:comment "clinic.  a medical facility associated with a hospital for outpatients"@en ;
      rdfs:subClassOf ontologyofspatialobject:Spot .

ontologyofspatialobject:flat
      a       owl:Class ;
      rdfs:comment "flat.  a small level or nearly level area"@en ;
      rdfs:subClassOf ontologyofspatialobject:Undersea .

ontologyofspatialobject:Spot
      a       owl:Class ;
      rdfs:comment "S spot, building, farm"@en ;
      rdfs:subClassOf ontologyofspatialobject:GeonameConcept , ontologyofspatialobject:landmark .

ontologyofspatialobject:palace
      a       owl:Class ;
      rdfs:comment "palace.  a large stately house, often a royal or presidential residence"@en ;
      rdfs:subClassOf ontologyofspatialobject:Spot .

ontologyofspatialobject:mining-camp
      a       owl:Class ;
      rdfs:comment "mining camp.  a camp used by miners"@en ;
      rdfs:subClassOf ontologyofspatialobject:Spot .

ontologyofspatialobject:ancient-road
      a       owl:Class ;
      rdfs:comment "ancient road.  the remains of a road used by ancient cultures"@en ;
      rdfs:subClassOf ontologyofspatialobject:Road .

ontologyofspatialobject:slide
      a       owl:Class ;
      rdfs:comment "slide.  a mound of earth material, at the base of a slope and the associated scoured area"@en ;
      rdfs:subClassOf ontologyofspatialobject:Hypsographic .

ontologyofspatialobject:tourism
      a       owl:Class ;
      rdfs:comment "This is used to map places and things of specific interest to tourists. For example these may be places to see, places to stay and things and places providing support. See the page titled Tourism(\"http://wiki.openstreetmap.org/wiki/Tourism\") for an introduction on its usage. "@en ;
      rdfs:subClassOf ontologyofspatialobject:SpatialObject .

ontologyofspatialobject:phosphate-works
      a       owl:Class ;
      rdfs:comment "phosphate works.  a facility for producing fertilizer"@en ;
      rdfs:subClassOf ontologyofspatialobject:Spot .

ontologyofspatialobject:cirques
      a       owl:Class ;
      rdfs:comment "cirques.  bowl-like hollows partially surrounded by cliffs or steep slopes at the head of a glaciated valley"@en ;
      rdfs:subClassOf ontologyofspatialobject:Hypsographic .

ontologyofspatialobject:dockyard
      a       owl:Class ;
      rdfs:comment "dockyard.  a facility for servicing, building, or repairing ships"@en ;
      rdfs:subClassOf ontologyofspatialobject:Spot .

ontologyofspatialobject:railroad-siding
      a       owl:Class ;
      rdfs:comment "railroad siding.  a short track parallel to and joining the main track"@en ;
      rdfs:subClassOf ontologyofspatialobject:Spot .

ontologyofspatialobject:local-government-office
      a       owl:Class ;
      rdfs:comment "local government office.  a facility housing local governmental offices, usually a city, town, or village hall"@en ;
      rdfs:subClassOf ontologyofspatialobject:Spot .

ontologyofspatialobject:pagoda
      a       owl:Class ;
      rdfs:comment "pagoda.  a tower-like storied structure, usually a Buddhist shrine"@en ;
      rdfs:subClassOf ontologyofspatialobject:Spot .

ontologyofspatialobject:tablemount--or-guyot-
      a       owl:Class ;
      rdfs:comment "tablemount (or guyot).  a seamount having a comparatively smooth, flat top"@en ;
      rdfs:subClassOf ontologyofspatialobject:Undersea .

ontologyofspatialobject:promontory--ies-
      a       owl:Class ;
      rdfs:comment "promontory(-ies).  a bluff or prominent hill overlooking or projecting into a lowland"@en ;
      rdfs:subClassOf ontologyofspatialobject:Hypsographic .

ontologyofspatialobject:historical-administrative-division
      a       owl:Class ;
      rdfs:comment "historical administrative division.  a former administrative division of a political entity, undifferentiated as to administrative level"@en ;
      rdfs:subClassOf ontologyofspatialobject:AdministrativeBoundary .

ontologyofspatialobject:radio-station
      a       owl:Class ;
      rdfs:comment "radio station.  a facility for producing and transmitting information by radio waves"@en ;
      rdfs:subClassOf ontologyofspatialobject:Spot .

ontologyofspatialobject:pyramid
      a       owl:Class ;
      rdfs:comment "pyramid.  an ancient massive structure of square ground plan with four triangular faces meeting at a point and used for enclosing tombs"@en ;
      rdfs:subClassOf ontologyofspatialobject:Spot .

ontologyofspatialobject:street
      a       owl:Class ;
      rdfs:comment "street.  a paved urban thoroughfare"@en ;
      rdfs:subClassOf ontologyofspatialobject:Road .

ontologyofspatialobject:oilfield
      a       owl:Class ;
      rdfs:comment "oilfield.  an area containing a subterranean store of petroleum of economic value"@en ;
      rdfs:subClassOf ontologyofspatialobject:Area .

ontologyofspatialobject:sand-area
      a       owl:Class ;
      rdfs:comment "sand area.  a tract of land covered with sand"@en ;
      rdfs:subClassOf ontologyofspatialobject:Hypsographic .

ontologyofspatialobject:point
      a       owl:Class ;
      rdfs:comment "point.  a tapering piece of land projecting into a body of water, less prominent than a cape"@en ;
      rdfs:subClassOf ontologyofspatialobject:Hypsographic .

ontologyofspatialobject:resthouse
      a       owl:Class ;
      rdfs:comment "resthouse.  a structure maintained for the rest and shelter of travelers"@en ;
      rdfs:subClassOf ontologyofspatialobject:Spot .

ontologyofspatialobject:bank
      a       owl:Class ;
      rdfs:comment "bank.  an elevation, typically located on a shelf, over which the depth of water is relatively shallow but sufficient for safe surface navigation"@en , "bank.  A business establishment in which money is kept for saving or commercial purposes or is invested, supplied for loans, or exchanged."@en ;
      rdfs:subClassOf ontologyofspatialobject:Spot , ontologyofspatialobject:Undersea .

ontologyofspatialobject:atomic-center
      a       owl:Class ;
      rdfs:comment "atomic center.  a facility where atomic research is carried out"@en ;
      rdfs:subClassOf ontologyofspatialobject:Spot .

ontologyofspatialobject:gold-mine-s-
      a       owl:Class ;
      rdfs:comment "gold mine(s).  a mine where gold ore, or alluvial gold is extracted"@en ;
      rdfs:subClassOf ontologyofspatialobject:Spot .

ontologyofspatialobject:cone-s-
      a       owl:Class ;
      rdfs:comment "cone(s).  a conical landform composed of mud or volcanic material"@en ;
      rdfs:subClassOf ontologyofspatialobject:Hypsographic .

ontologyofspatialobject:wadi-bend
      a       owl:Class ;
      rdfs:comment "wadi bend.  a conspicuously curved or bent segment of a wadi"@en ;
      rdfs:subClassOf ontologyofspatialobject:Hydrographic .

ontologyofspatialobject:rank
      a       owl:DatatypeProperty ;
      rdfs:comment "indication of the popularity or relevancy of an article. The rank is an integer number from 1 for the least popular articles to 100 for the most popular articles. It is calculated from the number of links pointing to an article and the article length. The articles are more or less evenly distributed over the 100 ranks."@en ;
      rdfs:domain ontologyofspatialobject:SpatialObject ;
      rdfs:range xsd:int ;
      rdfs:subPropertyOf ontologyofspatialobject:wikipediaDataProperty .

ontologyofspatialobject:garden-s-
      a       owl:Class ;
      rdfs:comment "garden(s).  an enclosure for displaying selected plant or animal life"@en ;
      rdfs:subClassOf ontologyofspatialobject:Spot .

ontologyofspatialobject:knolls
      a       owl:Class ;
      rdfs:comment "knolls.  elevations rising generally more than 500 meters and less than 1,000 meters and of limited extent across the summits"@en ;
      rdfs:subClassOf ontologyofspatialobject:Undersea .

ontologyofspatialobject:crater-lakes
      a       owl:Class ;
      rdfs:comment "crater lakes.  lakes in a crater or caldera"@en ;
      rdfs:subClassOf ontologyofspatialobject:Hydrographic .

ontologyofspatialobject:asphalt-lake
      a       owl:Class ;
      rdfs:comment "asphalt lake.  a small basin containing naturally occurring asphalt"@en ;
      rdfs:subClassOf ontologyofspatialobject:Hypsographic .

ontologyofspatialobject:reservation
      a       owl:Class ;
      rdfs:comment "reservation.  a tract of land set aside for aboriginal, tribal, or native populations"@en ;
      rdfs:subClassOf ontologyofspatialobject:Area .

ontologyofspatialobject:beaches
      a       owl:Class ;
      rdfs:comment "beaches.  a shore zone of coarse unconsolidated sediment that extends from the low-water line to the highest reach of storm waves"@en ;
      rdfs:subClassOf ontologyofspatialobject:Hypsographic .

ontologyofspatialobject:pool-s-
      a       owl:Class ;
      rdfs:comment "pool(s).   or a small body of standing water\""@en ;
      rdfs:subClassOf ontologyofspatialobject:Hydrographic .

ontologyofspatialobject:escarpment
      a       owl:Class ;
      rdfs:comment "escarpment.  a long line of cliffs or steep slopes separating level surfaces above and below"@en ;
      rdfs:subClassOf ontologyofspatialobject:Hypsographic .

ontologyofspatialobject:reefs
      a       owl:Class ;
      rdfs:comment "reefs.  surface-navigation hazards composed of consolidated material"@en ;
      rdfs:subClassOf ontologyofspatialobject:Undersea .

ontologyofspatialobject:petroleum-basin
      a       owl:Class ;
      rdfs:comment "petroleum basin.  an area underlain by an oil-rich structural basin"@en ;
      rdfs:subClassOf ontologyofspatialobject:Area .

ontologyofspatialobject:adminName1
      a       owl:FunctionalProperty , owl:DatatypeProperty ;
      rdfs:comment "adminName1"@en ;
      rdfs:domain ontologyofspatialobject:SpatialObject ;
      rdfs:range xsd:string ;
      rdfs:subPropertyOf ontologyofspatialobject:gonameDataProperty .

ontologyofspatialobject:shrine
      a       owl:Class ;
      rdfs:comment "shrine.  a structure or place memorializing a person or religious concept"@en ;
      rdfs:subClassOf ontologyofspatialobject:Spot .

ontologyofspatialobject:tunnel
      a       owl:Class ;
      rdfs:comment "tunnel.  a subterranean passageway for transportation"@en ;
      rdfs:subClassOf ontologyofspatialobject:Road .

ontologyofspatialobject:ruined-bridge
      a       owl:Class ;
      rdfs:comment "ruined bridge.  a destroyed or decayed bridge which is no longer functional"@en ;
      rdfs:subClassOf ontologyofspatialobject:Spot .

ontologyofspatialobject:badlands
      a       owl:Class ;
      rdfs:comment "badlands.  an area characterized by a maze of very closely spaced, deep, narrow, steep-sided ravines, and sharp crests and pinnacles"@en ;
      rdfs:subClassOf ontologyofspatialobject:Hypsographic .

ontologyofspatialobject:lava-area
      a       owl:Class ;
      rdfs:comment "lava area.  an area of solidified lava"@en ;
      rdfs:subClassOf ontologyofspatialobject:Hypsographic .

ontologyofspatialobject:park
      a       owl:Class ;
      rdfs:comment "park.  an area, often of forested land, maintained as a place of beauty, or for recreation"@en ;
      rdfs:subClassOf ontologyofspatialobject:Area .

ontologyofspatialobject:park-headquarters
      a       owl:Class ;
      rdfs:comment "park headquarters.  a park administrative facility"@en ;
      rdfs:subClassOf ontologyofspatialobject:Spot .

ontologyofspatialobject:intermittent-reservoir
      a       owl:Class ;
      rdfs:comment "intermittent reservoir.  "@en ;
      rdfs:subClassOf ontologyofspatialobject:Hydrographic .

ontologyofspatialobject:water-pumping-station
      a       owl:Class ;
      rdfs:comment "water pumping station.  a facility for pumping water from a major well or through a pipeline"@en ;
      rdfs:subClassOf ontologyofspatialobject:Spot .

ontologyofspatialobject:boundingBox
      a       owl:FunctionalProperty , owl:DatatypeProperty ;
      rdfs:comment "boundingBox"@en ;
      rdfs:domain ontologyofspatialobject:SpatialObject ;
      rdfs:range xsd:string ;
      rdfs:subPropertyOf ontologyofspatialobject:gonameDataProperty ;
      owl:propertyDisjointWith
              ontologyofspatialobject:name .

ontologyofspatialobject:knoll
      a       owl:Class ;
      rdfs:comment "knoll.  an elevation rising generally more than 500 meters and less than 1,000 meters and of limited extent across the summit"@en ;
      rdfs:subClassOf ontologyofspatialobject:Undersea .

ontologyofspatialobject:proximity
      a       owl:TransitiveProperty , owl:ObjectProperty , owl:SymmetricProperty ;
      rdfs:comment "proximity relations"@en ;
      rdfs:domain ontologyofspatialobject:SpatialObject ;
      rdfs:range ontologyofspatialobject:SpatialObject ;
      rdfs:subPropertyOf ontologyofspatialobject:spatial .

ontologyofspatialobject:retreat
      a       owl:Class ;
      rdfs:comment "retreat.  a place of temporary seclusion, especially for religious groups"@en ;
      rdfs:subClassOf ontologyofspatialobject:Spot .

ontologyofspatialobject:timezone
      a       owl:FunctionalProperty , owl:DatatypeProperty ;
      rdfs:comment "timezone"@en ;
      rdfs:domain ontologyofspatialobject:SpatialObject ;
      rdfs:range xsd:string ;
      rdfs:subPropertyOf ontologyofspatialobject:gonameDataProperty .

ontologyofspatialobject:trough
      a       owl:Class ;
      rdfs:comment "trough.  a long depression of the sea floor characteristically flat bottomed and steep sided, and normally shallower than a trench"@en ;
      rdfs:subClassOf ontologyofspatialobject:Undersea .

ontologyofspatialobject:section-of-plain
      a       owl:Class ;
      rdfs:comment "section of plain.  "@en ;
      rdfs:subClassOf ontologyofspatialobject:Hypsographic .

ontologyofspatialobject:Countries
      a       owl:Class ;
      rdfs:comment "Countries"@en ;
      rdfs:subClassOf ontologyofspatialobject:AdministrativeBoundary .

ontologyofspatialobject:wreck
      a       owl:Class ;
      rdfs:comment "wreck.  the site of the remains of a wrecked vessel"@en ;
      rdfs:subClassOf ontologyofspatialobject:Spot .

ontologyofspatialobject:spur
      a       owl:Class ;
      rdfs:comment "spur.  a subordinate elevation, ridge, or rise projecting outward from a larger feature"@en ;
      rdfs:subClassOf ontologyofspatialobject:Undersea .

ontologyofspatialobject:edbDataProperty
      a       owl:FunctionalProperty , owl:DatatypeProperty ;
      rdfs:comment "Es para representar todas las dataproperty que se extraen de una base de datos. Todas son funcionales porque la BD esta al menos en primera forma normal. Pero el rango no es posible expresarlo pues puede vanir cualquiera de los tipos de datos." ;
      rdfs:domain ontologyofspatialobject:SpatialObject ;
      rdfs:range rdfs:Literal ;
      rdfs:subPropertyOf owl:topDataProperty .

ontologyofspatialobject:spit
      a       owl:Class ;
      rdfs:comment "spit.  a narrow, straight or curved continuation of a beach into a waterbody"@en ;
      rdfs:subClassOf ontologyofspatialobject:Hypsographic .

ontologyofspatialobject:crater-lake
      a       owl:Class ;
      rdfs:comment "crater lake.  a lake in a crater or caldera"@en ;
      rdfs:subClassOf ontologyofspatialobject:Natural-watercourses , ontologyofspatialobject:Hydrographic .

ontologyofspatialobject:tidal-flat-s-
      a       owl:Class ;
      rdfs:comment "tidal flat(s).  a large flat area of mud or sand attached to the shore and alternately covered and uncovered by the tide"@en ;
      rdfs:subClassOf ontologyofspatialobject:Hydrographic .

ontologyofspatialobject:asylum
      a       owl:Class ;
      rdfs:comment "asylum.  a facility where the insane are cared for and protected"@en ;
      rdfs:subClassOf ontologyofspatialobject:Spot .

ontologyofspatialobject:AdministrativeBoundary
      a       owl:Class ;
      rdfs:comment "Administrative Boundary"@en ;
      rdfs:subClassOf ontologyofspatialobject:GeonameConcept , ontologyofspatialobject:boundary ;
      owl:equivalentClass ontologyofspatialobject:administrative .

ontologyofspatialobject:castle
      a       owl:Class ;
      rdfs:comment "castle.  a large fortified building or set of buildings"@en ;
      rdfs:subClassOf ontologyofspatialobject:Spot .

ontologyofspatialobject:amenity
      a       owl:Class ;
      rdfs:comment "Used to map facilities used by visitors and residents. For example: toilets, telephones, banks, pharmacies, cafes, parking and schools. See the page Amenity(\"http://wiki.openstreetmap.org/wiki/Amenities\") for an introduction on its usage."@en ;
      rdfs:subClassOf ontologyofspatialobject:SpatialObject .

ontologyofspatialobject:boundary-marker
      a       owl:Class ;
      rdfs:comment "boundary marker.  a fixture marking a point along a boundary"@en ;
      rdfs:subClassOf ontologyofspatialobject:Spot .

ontologyofspatialobject:boundary
      a       owl:Class ;
      rdfs:comment "These are used to describe administrative and other boundaries. See the page boundary(\"http://wiki.openstreetmap.org/wiki/Boundaries\") for an introduction on its usage."@en ;
      rdfs:subClassOf ontologyofspatialobject:SpatialObject .

ontologyofspatialobject:distributary--ies-
      a       owl:Class ;
      rdfs:comment "distributary(-ies).  a branch which flows away from the main stream, as in a delta or irrigation canal"@en ;
      rdfs:subClassOf ontologyofspatialobject:Hydrographic .

ontologyofspatialobject:reef-s-
      a       owl:Class ;
      rdfs:comment "reef(s).  a surface-navigation hazard composed of consolidated material"@en ;
      rdfs:subClassOf ontologyofspatialobject:Hydrographic .

ontologyofspatialobject:tundra
      a       owl:Class ;
      rdfs:comment "tundra.  a marshy, treeless, high latitude plain, dominated by mosses, lichens, and low shrub vegetation under permafrost conditions"@en ;
      rdfs:subClassOf ontologyofspatialobject:Vegetation .

ontologyofspatialobject:language
      a       owl:DatatypeProperty ;
      rdfs:comment "ISO language code of article text"@en ;
      rdfs:domain ontologyofspatialobject:SpatialObject ;
      rdfs:range xsd:string ;
      rdfs:subPropertyOf ontologyofspatialobject:wikipediaDataProperty .

ontologyofspatialobject:dry-stream-bed
      a       owl:Class ;
      rdfs:comment "dry stream bed.  a channel formerly containing the water of a stream"@en ;
      rdfs:subClassOf ontologyofspatialobject:Hypsographic .

[]    ontologyofspatialobject:license
              "http://purl.org/NET/rdflicense/allrightsreserved" .

ontologyofspatialobject:agricultural-reserve
      a       owl:Class ;
      rdfs:comment "agricultural reserve.  a tract of land reserved for agricultural reclamation and/or development"@en ;
      rdfs:subClassOf ontologyofspatialobject:Area .

ontologyofspatialobject:stony-desert
      a       owl:Class ;
      rdfs:comment "stony desert.  a desert plain characterized by a surface veneer of gravel and stones"@en ;
      rdfs:subClassOf ontologyofspatialobject:Hypsographic .

ontologyofspatialobject:abandoned-oil-well
      a       owl:Class ;
      rdfs:comment "abandoned oil well.  "@en ;
      rdfs:subClassOf ontologyofspatialobject:Spot .

ontologyofspatialobject:tree-s-
      a       owl:Class ;
      rdfs:comment "tree(s).  a conspicuous tree used as a landmark"@en ;
      rdfs:subClassOf ontologyofspatialobject:Vegetation .

ontologyofspatialobject:cuesta-s-
      a       owl:Class ;
      rdfs:comment "cuesta(s).  an asymmetric ridge formed on tilted strata"@en ;
      rdfs:subClassOf ontologyofspatialobject:Hypsographic .

ontologyofspatialobject:stream-bend
      a       owl:Class ;
      rdfs:comment "stream bend.  a conspicuously curved or bent segment of a stream"@en ;
      rdfs:subClassOf ontologyofspatialobject:Hydrographic .

ontologyofspatialobject:seat-of-a-third-order-administrative-division
      a       owl:Class ;
      rdfs:comment "seat of a third-order administrative division.  "@en ;
      rdfs:subClassOf ontologyofspatialobject:PopulatedPlace .

ontologyofspatialobject:market
      a       owl:Class ;
      rdfs:comment "market.  a place where goods are bought and sold at regular intervals"@en ;
      rdfs:subClassOf ontologyofspatialobject:Spot .

ontologyofspatialobject:abandoned-camp
      a       owl:Class ;
      rdfs:comment "abandoned camp.  "@en ;
      rdfs:subClassOf ontologyofspatialobject:Spot .

[]    a       owl:AllDisjointProperties ;
      owl:members (ontologyofspatialobject:adminCode1 ontologyofspatialobject:adminCode2 ontologyofspatialobject:adminCode3 ontologyofspatialobject:adminCode4 ontologyofspatialobject:adminCode5 ontologyofspatialobject:adminName1 ontologyofspatialobject:adminName2 ontologyofspatialobject:alternateNames ontologyofspatialobject:continentCode ontologyofspatialobject:countryCode ontologyofspatialobject:idOSM ontologyofspatialobject:language ontologyofspatialobject:latitude ontologyofspatialobject:longitude ontologyofspatialobject:timezone) .

ontologyofspatialobject:levee
      a       owl:Class ;
      rdfs:comment "levee.   often built up artificially to control floods\""@en , "levee.  an embankment bordering a canyon, valley, or seachannel"@en ;
      rdfs:subClassOf ontologyofspatialobject:Hypsographic , ontologyofspatialobject:Undersea .

ontologyofspatialobject:coast
      a       owl:Class ;
      rdfs:comment "coast.  a zone of variable width straddling the shoreline"@en ;
      rdfs:subClassOf ontologyofspatialobject:Area .

ontologyofspatialobject:sanatorium
      a       owl:Class ;
      rdfs:comment "sanatorium.  a facility where victims of physical or mental disorders are treated"@en ;
      rdfs:subClassOf ontologyofspatialobject:Spot .

ontologyofspatialobject:mole
      a       owl:Class ;
      rdfs:comment "mole.  a massive structure of masonry or large stones serving as a pier or breakwater"@en ;
      rdfs:subClassOf ontologyofspatialobject:Spot .

ontologyofspatialobject:Facilities
      a       owl:Class ;
      rdfs:subClassOf ontologyofspatialobject:Hydrographic .

ontologyofspatialobject:destroyed-populated-place
      a       owl:Class ;
      rdfs:comment "destroyed populated place.  a village, town or city destroyed by a natural disaster, or by war"@en ;
      rdfs:subClassOf ontologyofspatialobject:PopulatedPlace .

ontologyofspatialobject:fan
      a       owl:Class ;
      rdfs:comment "fan.  a relatively smooth feature normally sloping away from the lower termination of a canyon or canyon system"@en ;
      rdfs:subClassOf ontologyofspatialobject:Undersea .

[]    a       swrl:Imp ;
      swrl:body
              [ a       swrl:AtomList ;
                rdf:first
                        [ a       swrl:ClassAtom ;
                          swrl:argument1 <urn:swrl#x> ;
                          swrl:classPredicate ontologyofspatialobject:SpatialObject
                        ] ;
                rdf:rest
                        [ a       swrl:AtomList ;
                          rdf:first
                                  [ a       swrl:ClassAtom ;
                                    swrl:argument1 <urn:swrl#y> ;
                                    swrl:classPredicate ontologyofspatialobject:SpatialObject
                                  ] ;
                          rdf:rest
                                  [ a       swrl:AtomList ;
                                    rdf:first
                                            [ a       swrl:DatavaluedPropertyAtom ;
                                              swrl:argument1 <urn:swrl#x> ;
                                              swrl:argument2 <urn:swrl#latitudx> ;
                                              swrl:propertyPredicate
                                                      ontologyofspatialobject:latitude
                                            ] ;
                                    rdf:rest
                                            [ a       swrl:AtomList ;
                                              rdf:first
                                                      [ a       swrl:DatavaluedPropertyAtom ;
                                                        swrl:argument1 <urn:swrl#y> ;
                                                        swrl:argument2 <urn:swrl#latitudy> ;
                                                        swrl:propertyPredicate
                                                                ontologyofspatialobject:latitude
                                                      ] ;
                                              rdf:rest
                                                      [ a       swrl:AtomList ;
                                                        rdf:first
                                                                [ a       swrl:BuiltinAtom ;
                                                                  swrl:arguments (<urn:swrl#latitudy> <urn:swrl#latitudx>) ;
                                                                  swrl:builtin swrlb:greaterThan
                                                                ] ;
                                                        rdf:rest ()
                                                      ]
                                            ]
                                  ]
                        ]
              ] ;
      swrl:head
              [ a       swrl:AtomList ;
                rdf:first
                        [ a       swrl:IndividualPropertyAtom ;
                          swrl:argument1 <urn:swrl#y> ;
                          swrl:argument2 <urn:swrl#x> ;
                          swrl:propertyPredicate
                                  ontologyofspatialobject:isNorthOf
                        ] ;
                rdf:rest ()
              ] .

ontologyofspatialobject:railroad-stop
      a       owl:Class ;
      rdfs:comment "railroad stop.  a place lacking station facilities where trains stop to pick up and unload passengers and freight"@en ;
      rdfs:subClassOf ontologyofspatialobject:Spot .

ontologyofspatialobject:wadi
      a       owl:Class ;
      rdfs:comment "wadi.   found primarily in North Africa and the Middle East\""@en ;
      rdfs:subClassOf ontologyofspatialobject:Hydrographic .

ontologyofspatialobject:lake
      a       owl:Class ;
      rdfs:comment "lake.  a large inland body of standing water"@en ;
      rdfs:subClassOf ontologyofspatialobject:Natural-watercourses , ontologyofspatialobject:Hydrographic .

ontologyofspatialobject:section-of-reef
      a       owl:Class ;
      rdfs:comment "section of reef.  "@en ;
      rdfs:subClassOf ontologyofspatialobject:Hydrographic .

ontologyofspatialobject:trench
      a       owl:Class ;
      rdfs:comment "trench.  a long, narrow, characteristically very deep and asymmetrical depression of the sea floor, with relatively steep sides"@en ;
      rdfs:subClassOf ontologyofspatialobject:Undersea .

ontologyofspatialobject:ravine-s-
      a       owl:Class ;
      rdfs:comment "ravine(s).  a small, narrow, deep, steep-sided stream channel, smaller than a gorge"@en ;
      rdfs:subClassOf ontologyofspatialobject:Hydrographic .

ontologyofspatialobject:lagoons
      a       owl:Class ;
      rdfs:comment "lagoons.  shallow coastal waterbodies, completely or partly separated from a larger body of water by a barrier island, coral reef or other depositional feature"@en ;
      rdfs:subClassOf ontologyofspatialobject:Natural-watercourses , ontologyofspatialobject:Hydrographic .

ontologyofspatialobject:SpatialObject
      a       owl:Class ;
      rdfs:comment "Spatial Object"@en .

ontologyofspatialobject:third-order-administrative-division
      a       owl:Class ;
      rdfs:comment "third-order administrative division.  a subdivision of a second-order administrative division"@en ;
      rdfs:subClassOf ontologyofspatialobject:AdministrativeBoundary .

ontologyofspatialobject:isthmus
      a       owl:Class ;
      rdfs:comment "isthmus.  a narrow strip of land connecting two larger land masses and bordered by water"@en ;
      rdfs:subClassOf ontologyofspatialobject:Hypsographic .

ontologyofspatialobject:hammock-s-
      a       owl:Class ;
      rdfs:comment "hammock(s).  a patch of ground, distinct from and slightly above the surrounding plain or wetland. Often occurs in groups"@en ;
      rdfs:subClassOf ontologyofspatialobject:Hypsographic .

ontologyofspatialobject:landuse
      a       owl:Class ;
      rdfs:comment "This is used to describe the purpose for which an area of land is being used. See the page titled Landuse(\"http://wiki.openstreetmap.org/wiki/Landuse\") for an introduction on its usage."@en ;
      rdfs:subClassOf ontologyofspatialobject:Spot .

ontologyofspatialobject:tomb-s-
      a       owl:Class ;
      rdfs:comment "tomb(s).  a structure for interring bodies"@en ;
      rdfs:subClassOf ontologyofspatialobject:Spot .

ontologyofspatialobject:mining-area
      a       owl:Class ;
      rdfs:comment "mining area.  an area of mine sites where minerals and ores are extracted"@en ;
      rdfs:subClassOf ontologyofspatialobject:Area .

ontologyofspatialobject:sewage-treatment-plant
      a       owl:Class ;
      rdfs:comment "sewage treatment plant.  facility for the processing of sewage and/or wastewater"@en ;
      rdfs:subClassOf ontologyofspatialobject:Spot .

ontologyofspatialobject:intermittent-oxbow-lake
      a       owl:Class ;
      rdfs:comment "intermittent oxbow lake.  "@en ;
      rdfs:subClassOf ontologyofspatialobject:Hydrographic .

ontologyofspatialobject:casino
      a       owl:Class ;
      rdfs:comment "casino.  a building used for entertainment, especially gambling"@en ;
      rdfs:subClassOf ontologyofspatialobject:Spot .

ontologyofspatialobject:railroad-tunnel
      a       owl:Class ;
      rdfs:comment "railroad tunnel.  a tunnel through which a railroad passes"@en ;
      rdfs:subClassOf ontologyofspatialobject:Road .

ontologyofspatialobject:section-of-wadi
      a       owl:Class ;
      rdfs:comment "section of wadi.  "@en ;
      rdfs:subClassOf ontologyofspatialobject:Hydrographic .

ontologyofspatialobject:pine-grove
      a       owl:Class ;
      rdfs:comment "pine grove.  a planting of pine trees"@en ;
      rdfs:subClassOf ontologyofspatialobject:Vegetation .

ontologyofspatialobject:fan-s-
      a       owl:Class ;
      rdfs:comment "fan(s).  a fan-shaped wedge of coarse alluvium with apex merging with a mountain stream bed and the fan spreading out at a low angle slope onto an adjacent plain"@en ;
      rdfs:subClassOf ontologyofspatialobject:Hypsographic .

ontologyofspatialobject:isPartOf
      a       owl:FunctionalProperty , owl:TransitiveProperty , owl:ObjectProperty ;
      rdfs:comment "tiene un"@es ;
      rdfs:domain ontologyofspatialobject:SpatialObject ;
      rdfs:range ontologyofspatialobject:SpatialObject ;
      rdfs:subPropertyOf ontologyofspatialobject:mereological ;
      owl:propertyDisjointWith
              ontologyofspatialobject:isWholeOf .

ontologyofspatialobject:library
      a       owl:Class ;
      rdfs:comment "library.  A place in which information resources such as books are kept for reading, reference, or lending."@en ;
      rdfs:subClassOf ontologyofspatialobject:Spot .

ontologyofspatialobject:wharf--ves-
      a       owl:Class ;
      rdfs:comment "wharf(-ves).  a structure of open rather than solid construction along a shore or a bank which provides berthing for ships and cargo-handling facilities"@en ;
      rdfs:subClassOf ontologyofspatialobject:Spot .

ontologyofspatialobject:rockfall
      a       owl:Class ;
      rdfs:comment "rockfall.  an irregular mass of fallen rock at the base of a cliff or steep slope"@en ;
      rdfs:subClassOf ontologyofspatialobject:Hypsographic .

ontologyofspatialobject:railroad
      a       owl:Class ;
      rdfs:comment "railroad.  a permanent twin steel-rail track on which freight and passenger cars move long distances"@en ;
      rdfs:subClassOf ontologyofspatialobject:Road .

ontologyofspatialobject:battlefield
      a       owl:Class ;
      rdfs:comment "battlefield.  a site of a land battle of historical importance"@en ;
      rdfs:subClassOf ontologyofspatialobject:Area .

ontologyofspatialobject:parking-lot
      a       owl:Class ;
      rdfs:comment "parking lot.  an area used for parking vehicles"@en ;
      rdfs:subClassOf ontologyofspatialobject:Spot .

ontologyofspatialobject:bank-s-
      a       owl:Class ;
      rdfs:comment "bank(s).  an elevation, typically located on a shelf, over which the depth of water is relatively shallow but sufficient for most surface navigation"@en ;
      rdfs:subClassOf ontologyofspatialobject:Hydrographic .

ontologyofspatialobject:atoll-s-
      a       owl:Class ;
      rdfs:comment "atoll(s).  a ring-shaped coral reef which has closely spaced islands on it encircling a lagoon"@en ;
      rdfs:subClassOf ontologyofspatialobject:Hypsographic .

ontologyofspatialobject:abandoned-farm
      a       owl:Class ;
      rdfs:comment "abandoned farm.  "@en ;
      rdfs:subClassOf ontologyofspatialobject:Spot .

ontologyofspatialobject:brewery
      a       owl:Class ;
      rdfs:comment "brewery.  one or more buildings where beer is brewed"@en ;
      rdfs:subClassOf ontologyofspatialobject:Spot .

ontologyofspatialobject:spatial
      a       owl:TransitiveProperty , owl:ObjectProperty , owl:SymmetricProperty ;
      rdfs:comment "spatial relations"@en ;
      rdfs:domain ontologyofspatialobject:SpatialObject ;
      rdfs:range ontologyofspatialobject:SpatialObject .

ontologyofspatialobject:salt-lakes
      a       owl:Class ;
      rdfs:comment "salt lakes.  inland bodies of salt water with no outlet"@en ;
      rdfs:subClassOf ontologyofspatialobject:Hydrographic .

ontologyofspatialobject:convent
      a       owl:Class ;
      rdfs:comment "convent.  a building where a community of nuns lives in seclusion"@en ;
      rdfs:subClassOf ontologyofspatialobject:Spot .

ontologyofspatialobject:historical-first-order-administrative-division
      a       owl:Class ;
      rdfs:comment "historical first-order administrative division.  a former first-order administrative division"@en ;
      rdfs:subClassOf ontologyofspatialobject:AdministrativeBoundary .

ontologyofspatialobject:prison
      a       owl:Class ;
      rdfs:comment "prison.  a facility for confining prisoners"@en ;
      rdfs:subClassOf ontologyofspatialobject:Spot .

ontologyofspatialobject:anabranch
      a       owl:Class ;
      rdfs:comment "anabranch.  a diverging branch flowing out of a main stream and rejoining it downstream"@en ;
      rdfs:subClassOf ontologyofspatialobject:Hydrographic .

ontologyofspatialobject:fuel-depot
      a       owl:Class ;
      rdfs:comment "fuel depot.  an area where fuel is stored"@en ;
      rdfs:subClassOf ontologyofspatialobject:Spot .

ontologyofspatialobject:grave
      a       owl:Class ;
      rdfs:comment "grave.  a burial site"@en ;
      rdfs:subClassOf ontologyofspatialobject:Spot .

ontologyofspatialobject:dry-dock
      a       owl:Class ;
      rdfs:comment "dry dock.  a dock providing support for a vessel, and means for removing the water so that the bottom of the vessel can be exposed"@en ;
      rdfs:subClassOf ontologyofspatialobject:Spot .

ontologyofspatialobject:cove-s-
      a       owl:Class ;
      rdfs:comment "cove(s).  a small coastal indentation, smaller than a bay"@en ;
      rdfs:subClassOf ontologyofspatialobject:Hydrographic .

ontologyofspatialobject:drainage-canal
      a       owl:Class ;
      rdfs:comment "drainage canal.  an artificial waterway carrying water away from a wetland or from drainage ditches"@en ;
      rdfs:subClassOf ontologyofspatialobject:Hydrographic .

ontologyofspatialobject:section-of-bank
      a       owl:Class ;
      rdfs:comment "section of bank.  "@en ;
      rdfs:subClassOf ontologyofspatialobject:Hydrographic .

ontologyofspatialobject:aeroway
      a       owl:Class ;
      rdfs:comment "These are mainly related to aerodromes, airfields other ground facilities that support the operation of airplanes and helicopters. See the page Aeroway(\"http://wiki.openstreetmap.org/wiki/Aeroways\") for an introduction on mapping these features."@en ;
      rdfs:subClassOf ontologyofspatialobject:SpatialObject .

ontologyofspatialobject:beacon
      a       owl:Class ;
      rdfs:comment "beacon.  a fixed artificial navigation mark"@en ;
      rdfs:subClassOf ontologyofspatialobject:Spot .

ontologyofspatialobject:apron
      a       owl:Class ;
      rdfs:comment "apron.  a gentle slope, with a generally smooth surface, particularly found around groups of islands and seamounts"@en ;
      rdfs:subClassOf ontologyofspatialobject:Undersea .

ontologyofspatialobject:veterinary-facility
      a       owl:Class ;
      rdfs:comment "veterinary facility.  a building or camp at which veterinary services are available"@en ;
      rdfs:subClassOf ontologyofspatialobject:Spot .

ontologyofspatialobject:well
      a       owl:Class ;
      rdfs:comment "well.  a cylindrical hole, pit, or tunnel drilled or dug down to a depth from which water, oil, or gas can be pumped or brought to the surface"@en ;
      rdfs:subClassOf ontologyofspatialobject:Hydrographic .

ontologyofspatialobject:coast-guard-station
      a       owl:Class ;
      rdfs:comment "coast guard station.  a facility from which the coast is guarded by armed vessels"@en ;
      rdfs:subClassOf ontologyofspatialobject:Spot .

ontologyofspatialobject:salt-ponds
      a       owl:Class ;
      rdfs:comment "salt ponds.  small standing bodies of salt water often in a marsh or swamp, usually along a seacoast"@en ;
      rdfs:subClassOf ontologyofspatialobject:Hydrographic .

ontologyofspatialobject:border-post
      a       owl:Class ;
      rdfs:comment "border post.  a post or station at an international boundary for the regulation of movement of people and goods"@en ;
      rdfs:subClassOf ontologyofspatialobject:Spot .

ontologyofspatialobject:isNorthOf
      a       owl:TransitiveProperty , owl:ObjectProperty ;
      rdfs:comment "is North of"@es ;
      rdfs:domain ontologyofspatialobject:SpatialObject ;
      rdfs:range ontologyofspatialobject:SpatialObject ;
      rdfs:subPropertyOf ontologyofspatialobject:directional ;
      owl:inverseOf ontologyofspatialobject:isSouthOf ;
      owl:propertyDisjointWith
              ontologyofspatialobject:isSouthOf .

ontologyofspatialobject:nunatak
      a       owl:Class ;
      rdfs:comment "nunatak.  a rock or mountain peak protruding through glacial ice"@en ;
      rdfs:subClassOf ontologyofspatialobject:Hypsographic .

ontologyofspatialobject:cordillera
      a       owl:Class ;
      rdfs:comment "cordillera.  an entire mountain system including the subordinate ranges, interior plateaus, and basins"@en ;
      rdfs:subClassOf ontologyofspatialobject:Undersea .

ontologyofspatialobject:crater-s-
      a       owl:Class ;
      rdfs:comment "crater(s).  a generally circular saucer or bowl-shaped depression caused by volcanic or meteorite explosive action"@en ;
      rdfs:subClassOf ontologyofspatialobject:Hypsographic .

ontologyofspatialobject:intermittent-stream
      a       owl:Class ;
      rdfs:comment "intermittent stream.  "@en ;
      rdfs:subClassOf ontologyofspatialobject:Hydrographic .

ontologyofspatialobject:freely-associated-state
      a       owl:Class ;
      rdfs:comment "freely associated state.  "@en ;
      rdfs:subClassOf ontologyofspatialobject:AdministrativeBoundary .

ontologyofspatialobject:rubber-plantation
      a       owl:Class ;
      rdfs:comment "rubber plantation.  an estate which specializes in growing and tapping rubber trees"@en ;
      rdfs:subClassOf ontologyofspatialobject:Spot .

ontologyofspatialobject:seachannels
      a       owl:Class ;
      rdfs:comment "seachannels.  continuously sloping, elongated depressions commonly found in fans or plains and customarily bordered by levees on one or two sides"@en ;
      rdfs:subClassOf ontologyofspatialobject:Undersea .

ontologyofspatialobject:plain-s-
      a       owl:Class ;
      rdfs:comment "plain(s).  an extensive area of comparatively level to gently undulating land, lacking surface irregularities, and usually adjacent to a higher area"@en ;
      rdfs:subClassOf ontologyofspatialobject:Hypsographic .

ontologyofspatialobject:valleys
      a       owl:Class ;
      rdfs:comment "valleys.  elongated depressions usually traversed by a stream"@en , "valleys.  a relatively shallow, wide depression, the bottom of which usually has a continuous gradient"@en ;
      rdfs:subClassOf ontologyofspatialobject:Hypsographic , ontologyofspatialobject:Undersea .

ontologyofspatialobject:dock-s-
      a       owl:Class ;
      rdfs:comment "dock(s).  a waterway between two piers, or cut into the land for the berthing of ships"@en ;
      rdfs:subClassOf ontologyofspatialobject:Hydrographic .

ontologyofspatialobject:disjoint
      a       owl:TransitiveProperty , owl:ObjectProperty , owl:SymmetricProperty ;
      rdfs:comment """Two geometries are disjoint if they dont have any points in common. Disjoint is the inverse of Intersects. Disjoint is the most efficient operator and is guaranteed to work even on non-simple geometries.

http://esri.github.io/geometry-api-java/doc/Disjoint.html"""@en ;
      rdfs:domain ontologyofspatialobject:SpatialObject ;
      rdfs:range ontologyofspatialobject:SpatialObject ;
      rdfs:subPropertyOf ontologyofspatialobject:topological ;
      owl:propertyDisjointWith
              ontologyofspatialobject:touches , ontologyofspatialobject:inside , ontologyofspatialobject:overlap , ontologyofspatialobject:equal , ontologyofspatialobject:intersects .

ontologyofspatialobject:hamlet
      a       owl:Class ;
      rdfs:subClassOf ontologyofspatialobject:place .

ontologyofspatialobject:rise
      a       owl:Class ;
      rdfs:comment "rise.  a broad elevation that rises gently, and generally smoothly, from the sea floor"@en ;
      rdfs:subClassOf ontologyofspatialobject:Undersea .

ontologyofspatialobject:shoals
      a       owl:Class ;
      rdfs:comment "shoals.  hazards to surface navigation composed of unconsolidated material"@en ;
      rdfs:subClassOf ontologyofspatialobject:Undersea .

ontologyofspatialobject:fourth-order-administrative-division
      a       owl:Class ;
      rdfs:comment "fourth-order administrative division.  a subdivision of a third-order administrative division"@en ;
      rdfs:subClassOf ontologyofspatialobject:AdministrativeBoundary .

ontologyofspatialobject:corral-s-
      a       owl:Class ;
      rdfs:comment "corral(s).  a pen or enclosure for confining or capturing animals"@en ;
      rdfs:subClassOf ontologyofspatialobject:Spot .

ontologyofspatialobject:emergency
      a       owl:Class ;
      rdfs:comment "This is used to describe the location of emergency facilities and equipment. See the page Emergency(\"http://wiki.openstreetmap.org/wiki/Emergency\") for an introduction on its usage."@en ;
      rdfs:subClassOf ontologyofspatialobject:SpatialObject .

ontologyofspatialobject:road-tunnel
      a       owl:Class ;
      rdfs:comment "road tunnel.  a tunnel through which a road passes"@en ;
      rdfs:subClassOf ontologyofspatialobject:Road .

ontologyofspatialobject:mesa
      a       owl:Class ;
      rdfs:comment "mesa.  an isolated, extensive, flat-topped elevation on the shelf, with relatively steep sides"@en ;
      rdfs:subClassOf ontologyofspatialobject:Undersea .

ontologyofspatialobject:mission
      a       owl:Class ;
      rdfs:comment "mission.  a place characterized by dwellings, school, church, hospital and other facilities operated by a religious group for the purpose of providing charitable services and to propagate religion"@en ;
      rdfs:subClassOf ontologyofspatialobject:Spot .

ontologyofspatialobject:seat-of-a-second-order-administrative-division
      a       owl:Class ;
      rdfs:comment "seat of a second-order administrative division.  "@en ;
      rdfs:subClassOf ontologyofspatialobject:PopulatedPlace .

ontologyofspatialobject:shop
      a       owl:Class ;
      rdfs:comment "The shop tag is used as a place of business that has stocked goods for sale. See the page titled Shop(\"http://wiki.openstreetmap.org/wiki/Shop\") for an introduction on its usage."@en ;
      rdfs:subClassOf ontologyofspatialobject:Spot .

ontologyofspatialobject:religious-center
      a       owl:Class ;
      rdfs:comment "religious center.  a facility where more than one religious activity is carried out, e.g., retreat, school, monastery, worship"@en ;
      rdfs:subClassOf ontologyofspatialobject:Spot .

ontologyofspatialobject:directional
      a       owl:TransitiveProperty , owl:ObjectProperty , owl:SymmetricProperty ;
      rdfs:comment "Directional relations"@en ;
      rdfs:domain ontologyofspatialobject:SpatialObject ;
      rdfs:range ontologyofspatialobject:SpatialObject ;
      rdfs:subPropertyOf ontologyofspatialobject:spatial .

ontologyofspatialobject:sulphur-spring-s-
      a       owl:Class ;
      rdfs:comment "sulphur spring(s).  a place where sulphur ground water flows naturally out of the ground"@en ;
      rdfs:subClassOf ontologyofspatialobject:Hydrographic .

ontologyofspatialobject:leper-colony
      a       owl:Class ;
      rdfs:comment "leper colony.  a settled area inhabited by lepers in relative isolation"@en ;
      rdfs:subClassOf ontologyofspatialobject:Spot .

ontologyofspatialobject:islands
      a       owl:Class ;
      rdfs:comment "islands.  tracts of land, smaller than a continent, surrounded by water at high water"@en ;
      rdfs:subClassOf ontologyofspatialobject:Hypsographic .

ontologyofspatialobject:oil-pumping-station
      a       owl:Class ;
      rdfs:comment "oil pumping station.  a facility for pumping oil through a pipeline"@en ;
      rdfs:subClassOf ontologyofspatialobject:Spot .

ontologyofspatialobject:abandoned-railroad
      a       owl:Class ;
      rdfs:comment "abandoned railroad.  "@en ;
      rdfs:subClassOf ontologyofspatialobject:Road .

ontologyofspatialobject:nunataks
      a       owl:Class ;
      rdfs:comment "nunataks.  rocks or mountain peaks protruding through glacial ice"@en ;
      rdfs:subClassOf ontologyofspatialobject:Hypsographic .

ontologyofspatialobject:maneuver-area
      a       owl:Class ;
      rdfs:comment "maneuver area.  a tract of land where military field exercises are carried out"@en ;
      rdfs:subClassOf ontologyofspatialobject:Area .

ontologyofspatialobject:whaling-station
      a       owl:Class ;
      rdfs:comment "whaling station.  a facility for butchering whales and processing train oil"@en ;
      rdfs:subClassOf ontologyofspatialobject:Spot .

ontologyofspatialobject:steps
      a       owl:Class ;
      rdfs:comment "steps.  stones or slabs placed for ease in ascending or descending a steep slope"@en ;
      rdfs:subClassOf ontologyofspatialobject:Spot .

ontologyofspatialobject:rocks
      a       owl:Class ;
      rdfs:comment "rocks.  conspicuous, isolated rocky masses"@en ;
      rdfs:subClassOf ontologyofspatialobject:Hypsographic .

ontologyofspatialobject:peaks
      a       owl:Class ;
      rdfs:comment "peaks.  prominent elevations, part of a larger feature, either pointed or of very limited extent across the summit"@en , "peaks.  pointed elevations atop a mountain, ridge, or other hypsographic features"@en ;
      rdfs:subClassOf ontologyofspatialobject:Hypsographic , ontologyofspatialobject:Undersea .

ontologyofspatialobject:marina
      a       owl:Class ;
      rdfs:comment "marina.  a harbor facility for small boats, yachts, etc."@en ;
      rdfs:subClassOf ontologyofspatialobject:Spot .

ontologyofspatialobject:docking-basin
      a       owl:Class ;
      rdfs:comment "docking basin.  a part of a harbor where ships dock"@en ;
      rdfs:subClassOf ontologyofspatialobject:Hydrographic .

ontologyofspatialobject:Man-made-waterways
      a       owl:Class ;
      rdfs:subClassOf ontologyofspatialobject:Hydrographic .

ontologyofspatialobject:former-inlet
      a       owl:Class ;
      rdfs:comment "former inlet.  an inlet which has been filled in, or blocked by deposits"@en ;
      rdfs:subClassOf ontologyofspatialobject:Hydrographic .

ontologyofspatialobject:type
      a       owl:FunctionalProperty , owl:DatatypeProperty ;
      rdfs:comment "Para saber si es un Nodo, una Relacion o una Camino (Way)"@es ;
      rdfs:domain ontologyofspatialobject:SpatialObject ;
      rdfs:range xsd:string ;
      rdfs:subPropertyOf ontologyofspatialobject:osmDataProperty .

ontologyofspatialobject:abandoned-populated-place
      a       owl:Class ;
      rdfs:comment "abandoned populated place.  "@en ;
      rdfs:subClassOf ontologyofspatialobject:PopulatedPlace .

ontologyofspatialobject:office-building
      a       owl:Class ;
      rdfs:comment "office building.  commercial building where business and/or services are conducted"@en ;
      rdfs:subClassOf ontologyofspatialobject:Spot .

ontologyofspatialobject:scrubland
      a       owl:Class ;
      rdfs:comment "scrubland.  an area of low trees, bushes, and shrubs stunted by some environmental limitation"@en ;
      rdfs:subClassOf ontologyofspatialobject:Vegetation .

ontologyofspatialobject:resort
      a       owl:Class ;
      rdfs:comment "resort.  a specialized facility for vacation, health, or participation sports activities"@en ;
      rdfs:subClassOf ontologyofspatialobject:Spot .

ontologyofspatialobject:section-of-lagoon
      a       owl:Class ;
      rdfs:comment "section of lagoon.  "@en ;
      rdfs:subClassOf ontologyofspatialobject:Hydrographic .

ontologyofspatialobject:chrome-mine-s-
      a       owl:Class ;
      rdfs:comment "chrome mine(s).  a mine where chrome ore is extracted"@en ;
      rdfs:subClassOf ontologyofspatialobject:Spot .

<urn:swrl#x>
      a       swrl:Variable .

ontologyofspatialobject:rapids
      a       owl:Class ;
      rdfs:comment "rapids.  a turbulent section of a stream associated with a steep, irregular stream bed"@en ;
      rdfs:subClassOf ontologyofspatialobject:Hydrographic .

ontologyofspatialobject:underground-lake
      a       owl:Class ;
      rdfs:comment "underground lake.  a standing body of water in a cave"@en ;
      rdfs:subClassOf ontologyofspatialobject:Hydrographic .

ontologyofspatialobject:windmill
      a       owl:Class ;
      rdfs:comment "windmill.  a mill or water pump powered by wind"@en ;
      rdfs:subClassOf ontologyofspatialobject:Spot .

ontologyofspatialobject:railroad-junction
      a       owl:Class ;
      rdfs:comment "railroad junction.  a place where two or more railroad tracks join"@en ;
      rdfs:subClassOf ontologyofspatialobject:Road .

ontologyofspatialobject:copper-works
      a       owl:Class ;
      rdfs:comment "copper works.  a facility for processing copper ore"@en ;
      rdfs:subClassOf ontologyofspatialobject:Spot .

ontologyofspatialobject:experiment-station
      a       owl:Class ;
      rdfs:comment "experiment station.  a facility for carrying out experiments"@en ;
      rdfs:subClassOf ontologyofspatialobject:Spot .

ontologyofspatialobject:foundry
      a       owl:Class ;
      rdfs:comment "foundry.  a building or works where metal casting is carried out"@en ;
      rdfs:subClassOf ontologyofspatialobject:Spot .

owl:preferredNamespaceUri
      a       owl:AnnotationProperty .

ontologyofspatialobject:ridge-s-
      a       owl:Class ;
      rdfs:comment "ridge(s).  a long narrow elevation with steep sides, and a more or less continuous crest"@en ;
      rdfs:subClassOf ontologyofspatialobject:Hypsographic .

ontologyofspatialobject:name
      a       owl:FunctionalProperty , owl:DatatypeProperty ;
      rdfs:comment """name

Es utilizado por Geoanmes y la fuente \"Base de Datos\", para el nombre de cada objeto espacial."""@en ;
      rdfs:domain ontologyofspatialobject:SpatialObject ;
      rdfs:range xsd:string ;
      rdfs:subPropertyOf ontologyofspatialobject:gonameDataProperty .

<urn:swrl#y>
      a       swrl:Variable .

ontologyofspatialobject:basin
      a       owl:Class ;
      rdfs:comment "basin.  a depression more or less equidimensional in plan and of variable extent"@en ;
      rdfs:subClassOf ontologyofspatialobject:Undersea .

ontologyofspatialobject:abandoned-prison
      a       owl:Class ;
      rdfs:comment "abandoned prison.  "@en ;
      rdfs:subClassOf ontologyofspatialobject:Spot .

ontologyofspatialobject:canal-bend
      a       owl:Class ;
      rdfs:comment "canal bend.  a conspicuously curved or bent section of a canal"@en ;
      rdfs:subClassOf ontologyofspatialobject:Hydrographic .

ontologyofspatialobject:land-tied-island
      a       owl:Class ;
      rdfs:comment "land-tied island.  a coastal island connected to the mainland by barrier beaches, levees or dikes"@en ;
      rdfs:subClassOf ontologyofspatialobject:Hypsographic .

ontologyofspatialobject:road
      a       owl:Class ;
      rdfs:comment "road.  an open way with improved surface for transportation of animals, people and vehicles"@en ;
      rdfs:subClassOf ontologyofspatialobject:Road .

ontologyofspatialobject:dam
      a       owl:Class ;
      rdfs:comment "dam.  a barrier constructed across a stream to impound water"@en ;
      rdfs:subClassOf ontologyofspatialobject:Spot .

ontologyofspatialobject:housing-development
      a       owl:Class ;
      rdfs:comment "housing development.  a tract of land on which many houses of similar design are built according to a development plan"@en ;
      rdfs:subClassOf ontologyofspatialobject:Area .

ontologyofspatialobject:section-of-peninsula
      a       owl:Class ;
      rdfs:comment "section of peninsula.  "@en ;
      rdfs:subClassOf ontologyofspatialobject:Hypsographic .

ontologyofspatialobject:town
      a       owl:Class ;
      rdfs:subClassOf ontologyofspatialobject:place .

ontologyofspatialobject:zoo
      a       owl:Class ;
      rdfs:comment "zoo.  a zoological garden or park where wild animals are kept for exhibition"@en ;
      rdfs:subClassOf ontologyofspatialobject:Spot .

ontologyofspatialobject:drainage-basin
      a       owl:Class ;
      rdfs:comment "drainage basin.  an area drained by a stream"@en ;
      rdfs:subClassOf ontologyofspatialobject:Area .

ontologyofspatialobject:historical-fourth-order-administrative-division
      a       owl:Class ;
      rdfs:comment "historical fourth-order administrative division.  a former fourth-order administrative division"@en ;
      rdfs:subClassOf ontologyofspatialobject:AdministrativeBoundary .

ontologyofspatialobject:island
      a       owl:Class ;
      rdfs:comment "island.  a tract of land, smaller than a continent, surrounded by water at high water"@en ;
      rdfs:subClassOf ontologyofspatialobject:Hypsographic .

ontologyofspatialobject:populated-locality
      a       owl:Class ;
      rdfs:comment "populated locality.  an area similar to a locality but with a small group of dwellings or other buildings"@en ;
      rdfs:subClassOf ontologyofspatialobject:PopulatedPlace .

ontologyofspatialobject:abandoned-well
      a       owl:Class ;
      rdfs:comment "abandoned well.  "@en ;
      rdfs:subClassOf ontologyofspatialobject:Hydrographic .

ontologyofspatialobject:borderland
      a       owl:Class ;
      rdfs:comment "borderland.  a region adjacent to a continent, normally occupied by or bordering a shelf, that is highly irregular with depths well in excess of those typical of a shelf"@en ;
      rdfs:subClassOf ontologyofspatialobject:Undersea .

ontologyofspatialobject:stream-mouth-s-
      a       owl:Class ;
      rdfs:comment "stream mouth(s).  a place where a stream discharges into a lagoon, lake, or the sea"@en ;
      rdfs:subClassOf ontologyofspatialobject:Hydrographic .

ontologyofspatialobject:intermittent-salt-pond-s-
      a       owl:Class ;
      rdfs:comment "intermittent salt pond(s).  "@en ;
      rdfs:subClassOf ontologyofspatialobject:Hydrographic .

ontologyofspatialobject:courthouse
      a       owl:Class ;
      rdfs:comment "courthouse.  a building in which courts of law are held"@en ;
      rdfs:subClassOf ontologyofspatialobject:Spot .

ontologyofspatialobject:peat-cutting-area
      a       owl:Class ;
      rdfs:comment "peat cutting area.  an area where peat is harvested"@en ;
      rdfs:subClassOf ontologyofspatialobject:Area .

ontologyofspatialobject:geyser
      a       owl:Class ;
      rdfs:comment "geyser.  a type of hot spring with intermittent eruptions of jets of hot water and steam"@en ;
      rdfs:subClassOf ontologyofspatialobject:Hydrographic .

ontologyofspatialobject:abandoned-railroad-station
      a       owl:Class ;
      rdfs:comment "abandoned railroad station.  "@en ;
      rdfs:subClassOf ontologyofspatialobject:Spot .

ontologyofspatialobject:rock
      a       owl:Class ;
      rdfs:comment "rock.  a conspicuous, isolated rocky mass"@en ;
      rdfs:subClassOf ontologyofspatialobject:Hypsographic .

ontologyofspatialobject:canalized-stream
      a       owl:Class ;
      rdfs:comment "canalized stream.  a stream that has been substantially ditched, diked, or straightened"@en ;
      rdfs:subClassOf ontologyofspatialobject:Hydrographic .

ontologyofspatialobject:canal-tunnel
      a       owl:Class ;
      rdfs:comment "canal tunnel.  a tunnel through which a canal passes"@en ;
      rdfs:subClassOf ontologyofspatialobject:Hydrographic .

ontologyofspatialobject:museum
      a       owl:Class ;
      rdfs:comment "museum.  a building where objects of permanent interest in one or more of the arts and sciences are preserved and exhibited"@en ;
      rdfs:subClassOf ontologyofspatialobject:Spot .

ontologyofspatialobject:clearing
      a       owl:Class ;
      rdfs:comment "clearing.  an area in a forest with trees removed"@en ;
      rdfs:subClassOf ontologyofspatialobject:Area .

ontologyofspatialobject:athletic-field
      a       owl:Class ;
      rdfs:comment "athletic field.  a tract of land used for playing team sports, and athletic track and field events"@en ;
      rdfs:subClassOf ontologyofspatialobject:sport , ontologyofspatialobject:Spot .

ontologyofspatialobject:wells
      a       owl:Class ;
      rdfs:comment "wells.  cylindrical holes, pits, or tunnels drilled or dug down to a depth from which water, oil, or gas can be pumped or brought to the surface"@en ;
      rdfs:subClassOf ontologyofspatialobject:Hydrographic .

ontologyofspatialobject:abandoned-factory
      a       owl:Class ;
      rdfs:comment "abandoned factory.  "@en ;
      rdfs:subClassOf ontologyofspatialobject:Spot .

ontologyofspatialobject:landmark
      a       owl:Class ;
      rdfs:comment "buildings (including churches, factories, museums, theatres, and power plants but excluding schools and railway stations), caves, cemeteries, cultural landmarks, geologic faults, headlands, intersections, mines, ranches, roads, structures (including antennas, bridges, castles, dams, lighthouses, monuments, and stadiums), tourist attractions, valleys, and other points of interest"@en ;
      rdfs:subClassOf ontologyofspatialobject:SpatialObject .

ontologyofspatialobject:mill-s-
      a       owl:Class ;
      rdfs:comment "mill(s).  a building housing machines for transforming, shaping, finishing, grinding, or extracting products"@en ;
      rdfs:subClassOf ontologyofspatialobject:Spot .

ontologyofspatialobject:route
      a       owl:Class ;
      rdfs:comment "This is used to describe routes of all different kinds. See the page titled Relation:route(\"http://wiki.openstreetmap.org/wiki/Relation:route\") for an introduction on its usage."@en ;
      rdfs:subClassOf ontologyofspatialobject:Road .

ontologyofspatialobject:not-available
      a       owl:Class ;
      rdfs:comment "not available.  "@en ;
      rdfs:subClassOf ontologyofspatialobject:Vegetation .

ontologyofspatialobject:countryCode
      a       owl:FunctionalProperty , owl:DatatypeProperty ;
      rdfs:comment "countryCode"@en ;
      rdfs:domain ontologyofspatialobject:SpatialObject ;
      rdfs:range xsd:string ;
      rdfs:subPropertyOf ontologyofspatialobject:gonameDataProperty .

ontologyofspatialobject:fishponds
      a       owl:Class ;
      rdfs:comment "fishponds.  ponds or enclosures in which fish are kept or raised"@en ;
      rdfs:subClassOf ontologyofspatialobject:Hydrographic .

ontologyofspatialobject:scientific-research-base
      a       owl:Class ;
      rdfs:comment "scientific research base.  a scientific facility used as a base from which research is carried out or monitored"@en ;
      rdfs:subClassOf ontologyofspatialobject:Spot .

ontologyofspatialobject:bench
      a       owl:Class ;
      rdfs:comment "bench.  a long, narrow bedrock platform bounded by steeper slopes above and below, usually overlooking a waterbody"@en ;
      rdfs:subClassOf ontologyofspatialobject:Hypsographic .

ontologyofspatialobject:stadium
      a       owl:Class ;
      rdfs:comment "stadium.  a structure with an enclosure for athletic games with tiers of seats for spectators"@en ;
      rdfs:subClassOf ontologyofspatialobject:Spot .

ontologyofspatialobject:section-of-valley
      a       owl:Class ;
      rdfs:comment "section of valley.  "@en ;
      rdfs:subClassOf ontologyofspatialobject:Hypsographic .

ontologyofspatialobject:historical-site
      a       owl:Class ;
      rdfs:comment "historical site.  a place of historical importance"@en ;
      rdfs:subClassOf ontologyofspatialobject:Spot .

ontologyofspatialobject:spillway
      a       owl:Class ;
      rdfs:comment "spillway.  a passage or outlet through which surplus water flows over, around or through a dam"@en ;
      rdfs:subClassOf ontologyofspatialobject:Spot .

ontologyofspatialobject:plateau
      a       owl:Class ;
      rdfs:comment "plateau.  a comparatively flat-topped feature of considerable extent, dropping off abruptly on one or more sides"@en , "plateau.  an elevated plain with steep slopes on one or more sides, and often with incised streams"@en ;
      rdfs:subClassOf ontologyofspatialobject:Hypsographic , ontologyofspatialobject:Undersea .

ontologyofspatialobject:section-of-canal
      a       owl:Class ;
      rdfs:comment "section of canal.  "@en ;
      rdfs:subClassOf ontologyofspatialobject:Hydrographic .

ontologyofspatialobject:square
      a       owl:Class ;
      rdfs:comment "square.  a broad, open, public area near the center of a town or city"@en ;
      rdfs:subClassOf ontologyofspatialobject:Spot .

ontologyofspatialobject:sugar-refinery
      a       owl:Class ;
      rdfs:comment "sugar refinery.  a facility for converting raw sugar into refined sugar"@en ;
      rdfs:subClassOf ontologyofspatialobject:Spot .

ontologyofspatialobject:hydroelectric-power-station
      a       owl:Class ;
      rdfs:comment "hydroelectric power station.  a building where electricity is generated from water power"@en ;
      rdfs:subClassOf ontologyofspatialobject:Spot .

ontologyofspatialobject:seamount
      a       owl:Class ;
      rdfs:comment "seamount.  an elevation rising generally more than 1,000 meters and of limited extent across the summit"@en ;
      rdfs:subClassOf ontologyofspatialobject:Undersea .

ontologyofspatialobject:military-school
      a       owl:Class ;
      rdfs:comment "military school.  a school at which military science forms the core of the curriculum"@en ;
      rdfs:subClassOf ontologyofspatialobject:Spot .

ontologyofspatialobject:watercourse
      a       owl:Class ;
      rdfs:comment "watercourse.  a natural, well-defined channel produced by flowing water, or an artificial channel designed to carry flowing water"@en ;
      rdfs:subClassOf ontologyofspatialobject:Hydrographic .

ontologyofspatialobject:isFarOf
      a       owl:ObjectProperty , owl:SymmetricProperty ;
      rdfs:comment "Is far of"@en ;
      rdfs:domain ontologyofspatialobject:SpatialObject ;
      rdfs:range ontologyofspatialobject:SpatialObject ;
      rdfs:subPropertyOf ontologyofspatialobject:proximity ;
      owl:propertyDisjointWith
              ontologyofspatialobject:isNearOf .

ontologyofspatialobject:israeli-settlement
      a       owl:Class ;
      rdfs:comment "israeli settlement.  "@en ;
      rdfs:subClassOf ontologyofspatialobject:PopulatedPlace .

ontologyofspatialobject:rock-desert
      a       owl:Class ;
      rdfs:comment "rock desert.  a relatively sand-free, high bedrock plateau in a hot desert, with or without a gravel veneer"@en ;
      rdfs:subClassOf ontologyofspatialobject:Hypsographic .

ontologyofspatialobject:arrugado
      a       owl:Class ;
      rdfs:comment "arrugado.  an area of subdued corrugations off Baja California"@en ;
      rdfs:subClassOf ontologyofspatialobject:Undersea .

ontologyofspatialobject:road-bend
      a       owl:Class ;
      rdfs:comment "road bend.  a conspicuously curved or bent section of a road"@en ;
      rdfs:subClassOf ontologyofspatialobject:Road .

ontologyofspatialobject:saddle
      a       owl:Class ;
      rdfs:comment "saddle.  a broad, open pass crossing a ridge or between hills or mountains"@en , "saddle.  a low part, resembling in shape a saddle, in a ridge or between contiguous seamounts"@en ;
      rdfs:subClassOf ontologyofspatialobject:Hypsographic , ontologyofspatialobject:Undersea .

ontologyofspatialobject:forest-reserve
      a       owl:Class ;
      rdfs:comment "forest reserve.  a forested area set aside for preservation or controlled use"@en ;
      rdfs:subClassOf ontologyofspatialobject:Area .

ontologyofspatialobject:Undersea
      a       owl:Class ;
      rdfs:comment "U undersea"@en ;
      rdfs:subClassOf ontologyofspatialobject:GeonameConcept .

ontologyofspatialobject:customs-post
      a       owl:Class ;
      rdfs:comment "customs post.  a building at an international boundary where customs and duties are paid on goods"@en ;
      rdfs:subClassOf ontologyofspatialobject:Spot .

ontologyofspatialobject:isWholeOf
      a       owl:TransitiveProperty , owl:ObjectProperty ;
      rdfs:comment "Tiene varios"@es ;
      rdfs:domain ontologyofspatialobject:SpatialObject ;
      rdfs:range ontologyofspatialobject:SpatialObject ;
      rdfs:subPropertyOf ontologyofspatialobject:mereological ;
      owl:inverseOf ontologyofspatialobject:isPartOf .

ontologyofspatialobject:mall
      a       owl:Class ;
      rdfs:comment "mall.  A large, often enclosed shopping complex containing various stores, businesses, and restaurants usually accessible by common passageways."@en ;
      rdfs:subClassOf ontologyofspatialobject:shop , ontologyofspatialobject:Spot .

ontologyofspatialobject:interfluve
      a       owl:Class ;
      rdfs:comment "interfluve.  a relatively undissected upland between adjacent stream valleys"@en ;
      rdfs:subClassOf ontologyofspatialobject:Hypsographic .

ontologyofspatialobject:intermittent-lakes
      a       owl:Class ;
      rdfs:comment "intermittent lakes.  "@en ;
      rdfs:subClassOf ontologyofspatialobject:Hydrographic .

ontologyofspatialobject:harbor-s-
      a       owl:Class ;
      rdfs:comment "harbor(s).  a haven or space of deep water so sheltered by the adjacent land as to afford a safe anchorage for ships"@en ;
      rdfs:subClassOf ontologyofspatialobject:Hydrographic .

ontologyofspatialobject:underground-irrigation-canal-s-
      a       owl:Class ;
      rdfs:comment "underground irrigation canal(s).  a gently inclined underground tunnel bringing water for irrigation from aquifers"@en ;
      rdfs:subClassOf ontologyofspatialobject:Hydrographic .

ontologyofspatialobject:religious-populated-place
      a       owl:Class ;
      rdfs:comment "religious populated place.  a populated place whose population is largely engaged in religious occupations"@en ;
      rdfs:subClassOf ontologyofspatialobject:PopulatedPlace .

ontologyofspatialobject:gorge-s-
      a       owl:Class ;
      rdfs:comment "gorge(s).  a short, narrow, steep-sided section of a stream valley"@en ;
      rdfs:subClassOf ontologyofspatialobject:Hypsographic .

ontologyofspatialobject:feature
      a       owl:DatatypeProperty ;
      rdfs:comment "the wikipedia feature type. A list of types is available here: http://www.geonames.org/wikipedia/wikipedia_features.html"@en ;
      rdfs:domain ontologyofspatialobject:SpatialObject ;
      rdfs:range xsd:string ;
      rdfs:subPropertyOf ontologyofspatialobject:wikipediaDataProperty .

ontologyofspatialobject:Vegetation
      a       owl:Class ;
      rdfs:comment "Vegetation"@en ;
      rdfs:subClassOf ontologyofspatialobject:GeonameConcept , ontologyofspatialobject:natural .

ontologyofspatialobject:nature-reserve
      a       owl:Class ;
      rdfs:comment "nature reserve.  an area reserved for the maintenance of a natural habitat"@en ;
      rdfs:subClassOf ontologyofspatialobject:Area .

ontologyofspatialobject:post-office
      a       owl:Class ;
      rdfs:comment "post office.  a public building in which mail is received, sorted and distributed"@en ;
      rdfs:subClassOf ontologyofspatialobject:Spot .

ontologyofspatialobject:railroad-station
      a       owl:Class ;
      rdfs:comment "railroad station.  a facility comprising ticket office, platforms, etc. for loading and unloading train passengers and freight"@en ;
      rdfs:subClassOf ontologyofspatialobject:Spot .

ontologyofspatialobject:patrol-post
      a       owl:Class ;
      rdfs:comment "patrol post.  a post from which patrols are sent out"@en ;
      rdfs:subClassOf ontologyofspatialobject:Spot .

ontologyofspatialobject:ocean
      a       owl:Class ;
      rdfs:comment "ocean.  one of the major divisions of the vast expanse of salt water covering part of the earth"@en ;
      rdfs:subClassOf ontologyofspatialobject:Natural-watercourses , ontologyofspatialobject:Hydrographic .

ontologyofspatialobject:airport
      a       owl:Class ;
      rdfs:comment "airport.  a place where aircraft regularly land and take off, with runways, navigational aids, and major facilities for the commercial handling of passengers and cargo"@en ;
      rdfs:subClassOf ontologyofspatialobject:Spot , ontologyofspatialobject:aerodrome .

ontologyofspatialobject:historical-third-order-administrative-division
      a       owl:Class ;
      rdfs:comment "historical third-order administrative division.  a former third-order administrative division"@en ;
      rdfs:subClassOf ontologyofspatialobject:AdministrativeBoundary .

ontologyofspatialobject:highway
      a       owl:Class ;
      rdfs:comment "This is used to describe roads and footpaths. For an introduction on its usage see the page titled Highways(\"http://wiki.openstreetmap.org/wiki/Highways\"). See the page titled Restrictions for an introduction on access limitations by vehicles type, time, day, load and purpose, etc. "@en ;
      rdfs:subClassOf ontologyofspatialobject:Road .

owl:title
      a       owl:AnnotationProperty .

ontologyofspatialobject:escarpment--or-scarp-
      a       owl:Class ;
      rdfs:comment "escarpment (or scarp).  an elongated and comparatively steep slope separating flat or gently sloping areas"@en ;
      rdfs:subClassOf ontologyofspatialobject:Undersea .

ontologyofspatialobject:peninsula
      a       owl:Class ;
      rdfs:comment "peninsula.  an elongate area of land projecting into a body of water and nearly surrounded by water"@en ;
      rdfs:subClassOf ontologyofspatialobject:Hypsographic .

ontologyofspatialobject:leisure
      a       owl:Class ;
      rdfs:comment "This is used to tag leisure and sports facilities. See the page titled Leisure(\"http://wiki.openstreetmap.org/wiki/Leisure\") for an introduction on its usage."@en ;
      rdfs:subClassOf ontologyofspatialobject:Spot .

ontologyofspatialobject:lakes
      a       owl:Class ;
      rdfs:comment "lakes.  large inland bodies of standing water"@en ;
      rdfs:subClassOf ontologyofspatialobject:Hydrographic .

ontologyofspatialobject:ruined-dam
      a       owl:Class ;
      rdfs:comment "ruined dam.  a destroyed or decayed dam which is no longer functional"@en ;
      rdfs:subClassOf ontologyofspatialobject:Spot .

ontologyofspatialobject:irrigation-canal
      a       owl:Class ;
      rdfs:comment "irrigation canal.  a canal which serves as a main conduit for irrigation water"@en ;
      rdfs:subClassOf ontologyofspatialobject:Hydrographic .

ontologyofspatialobject:caravan-route
      a       owl:Class ;
      rdfs:comment "caravan route.  the route taken by caravans"@en ;
      rdfs:subClassOf ontologyofspatialobject:Road .

ontologyofspatialobject:dairy
      a       owl:Class ;
      rdfs:comment "dairy.  a facility for the processing, sale and distribution of milk or milk products"@en ;
      rdfs:subClassOf ontologyofspatialobject:Spot .

ontologyofspatialobject:seachannel
      a       owl:Class ;
      rdfs:comment "seachannel.  a continuously sloping, elongated depression commonly found in fans or plains and customarily bordered by levees on one or two sides"@en ;
      rdfs:subClassOf ontologyofspatialobject:Undersea .

ontologyofspatialobject:parish
      a       owl:Class ;
      rdfs:comment "parish.  an ecclesiastical district"@en ;
      rdfs:subClassOf ontologyofspatialobject:AdministrativeBoundary .

ontologyofspatialobject:hot-spring-s-
      a       owl:Class ;
      rdfs:comment "hot spring(s).  a place where hot ground water flows naturally out of the ground"@en ;
      rdfs:subClassOf ontologyofspatialobject:Hydrographic .

ontologyofspatialobject:summary
      a       owl:DatatypeProperty ;
      rdfs:comment "a short summary of the article text. Around 300 chars. The text is truncated at a full stop if one is available near char 300, otherwise at the end of a word."@en ;
      rdfs:domain ontologyofspatialobject:SpatialObject ;
      rdfs:range xsd:string ;
      rdfs:subPropertyOf ontologyofspatialobject:wikipediaDataProperty .

ontologyofspatialobject:furrow
      a       owl:Class ;
      rdfs:comment "furrow.  a closed, linear, narrow, shallow depression"@en ;
      rdfs:subClassOf ontologyofspatialobject:Undersea .

ontologyofspatialobject:isEastOf
      a       owl:TransitiveProperty , owl:ObjectProperty ;
      rdfs:comment "is East Of"@es ;
      rdfs:domain ontologyofspatialobject:SpatialObject ;
      rdfs:range ontologyofspatialobject:SpatialObject ;
      rdfs:subPropertyOf ontologyofspatialobject:directional ;
      owl:inverseOf ontologyofspatialobject:isWestOf ;
      owl:propertyDisjointWith
              ontologyofspatialobject:isWestOf .

ontologyofspatialobject:seat-of-government-of-a-political-entity
      a       owl:Class ;
      rdfs:comment "seat of government of a political entity.  "@en ;
      rdfs:subClassOf ontologyofspatialobject:PopulatedPlace .

ontologyofspatialobject:lake-region
      a       owl:Class ;
      rdfs:comment "lake region.  a tract of land distinguished by numerous lakes"@en ;
      rdfs:subClassOf ontologyofspatialobject:Area .

ontologyofspatialobject:intermittent-salt-lakes
      a       owl:Class ;
      rdfs:comment "intermittent salt lakes.  "@en ;
      rdfs:subClassOf ontologyofspatialobject:Hydrographic .

[]    a       swrl:Imp ;
      swrl:body
              [ a       swrl:AtomList ;
                rdf:first
                        [ a       swrl:BuiltinAtom ;
                          swrl:arguments
                                  [ a       rdf:List ;
                                    rdf:first <urn:swrl#latitud> ;
                                    rdf:rest
                                            [ a       rdf:List ;
                                              rdf:first 0 ;
                                              rdf:rest ()
                                            ]
                                  ] ;
                          swrl:builtin swrlb:greaterThan
                        ] ;
                rdf:rest
                        [ a       swrl:AtomList ;
                          rdf:first
                                  [ a       swrl:DatavaluedPropertyAtom ;
                                    swrl:argument1 <urn:swrl#x> ;
                                    swrl:argument2 <urn:swrl#latitud> ;
                                    swrl:propertyPredicate
                                            ontologyofspatialobject:latitude
                                  ] ;
                          rdf:rest
                                  [ a       swrl:AtomList ;
                                    rdf:first
                                            [ a       swrl:ClassAtom ;
                                              swrl:argument1 <urn:swrl#x> ;
                                              swrl:classPredicate ontologyofspatialobject:SpatialObject
                                            ] ;
                                    rdf:rest ()
                                  ]
                        ]
              ] ;
      swrl:head
              [ a       swrl:AtomList ;
                rdf:first
                        [ a       swrl:ClassAtom ;
                          swrl:argument1 <urn:swrl#x> ;
                          swrl:classPredicate ontologyofspatialobject:NortHemisphere
                        ] ;
                rdf:rest ()
              ] .

ontologyofspatialobject:vineyard
      a       owl:Class ;
      rdfs:comment "vineyard.  a planting of grapevines"@en ;
      rdfs:subClassOf ontologyofspatialobject:Vegetation .

ontologyofspatialobject:jetty
      a       owl:Class ;
      rdfs:comment "jetty.  a structure built out into the water at a river mouth or harbor entrance to regulate currents and silting"@en ;
      rdfs:subClassOf ontologyofspatialobject:Spot .

ontologyofspatialobject:section-of-independent-political-entity
      a       owl:Class ;
      rdfs:comment "section of independent political entity.  "@en ;
      rdfs:subClassOf ontologyofspatialobject:AdministrativeBoundary .

ontologyofspatialobject:second-order-administrative-division
      a       owl:Class ;
      rdfs:comment "second-order administrative division.  a subdivision of a first-order administrative division"@en ;
      rdfs:subClassOf ontologyofspatialobject:AdministrativeBoundary .

ontologyofspatialobject:topological
      a       owl:TransitiveProperty , owl:ObjectProperty , owl:SymmetricProperty ;
      rdfs:comment "topological relations"@en ;
      rdfs:domain ontologyofspatialobject:SpatialObject ;
      rdfs:range ontologyofspatialobject:SpatialObject ;
      rdfs:subPropertyOf ontologyofspatialobject:spatial .

ontologyofspatialobject:channel
      a       owl:Class ;
      rdfs:comment "channel.  the deepest part of a stream, bay, lagoon, or strait, through which the main current flows"@en ;
      rdfs:subClassOf ontologyofspatialobject:Natural-watercourses , ontologyofspatialobject:Hydrographic .

ontologyofspatialobject:bus-stop
      a       owl:Class ;
      rdfs:comment "bus stop.  a place lacking station facilities"@en ;
      rdfs:subClassOf ontologyofspatialobject:Spot .

ontologyofspatialobject:fissure
      a       owl:Class ;
      rdfs:comment "fissure.  a crack associated with volcanism"@en ;
      rdfs:subClassOf ontologyofspatialobject:Hypsographic .

ontologyofspatialobject:isWestOf
      a       owl:TransitiveProperty , owl:ObjectProperty ;
      rdfs:comment "is West of"@en ;
      rdfs:domain ontologyofspatialobject:SpatialObject ;
      rdfs:range ontologyofspatialobject:SpatialObject ;
      rdfs:subPropertyOf ontologyofspatialobject:directional .

ontologyofspatialobject:grassland
      a       owl:Class ;
      rdfs:comment "grassland.  an area dominated by grass vegetation"@en ;
      rdfs:subClassOf ontologyofspatialobject:Vegetation .

ontologyofspatialobject:administrative-facility
      a       owl:Class ;
      rdfs:comment "administrative facility.  a government building"@en ;
      rdfs:subClassOf ontologyofspatialobject:Spot .

ontologyofspatialobject:place
      a       owl:Class ;
      rdfs:comment "This is used mainly to give details about settlements. See the page titled Place(\"http://wiki.openstreetmap.org/wiki/Places\") for an introduction on its usage."@en ;
      rdfs:subClassOf ontologyofspatialobject:SpatialObject .

ontologyofspatialobject:amphitheater
      a       owl:Class ;
      rdfs:comment "amphitheater.  an oval or circular structure with rising tiers of seats about a stage or open space"@en ;
      rdfs:subClassOf ontologyofspatialobject:Spot .

ontologyofspatialobject:temple-s-
      a       owl:Class ;
      rdfs:comment "temple(s).  an edifice dedicated to religious worship"@en ;
      rdfs:subClassOf ontologyofspatialobject:Spot .

ontologyofspatialobject:ridges
      a       owl:Class ;
      rdfs:comment "ridges.  long narrow elevations with steep sides"@en ;
      rdfs:subClassOf ontologyofspatialobject:Undersea .

ontologyofspatialobject:mangrove-swamp
      a       owl:Class ;
      rdfs:comment "mangrove swamp.  a tropical tidal mud flat characterized by mangrove vegetation"@en ;
      rdfs:subClassOf ontologyofspatialobject:Hydrographic .

ontologyofspatialobject:bog-s-
      a       owl:Class ;
      rdfs:comment "bog(s).  a wetland characterized by peat forming sphagnum moss, sedge, and other acid-water plants"@en ;
      rdfs:subClassOf ontologyofspatialobject:Hydrographic .

ontologyofspatialobject:hermitage
      a       owl:Class ;
      rdfs:comment "hermitage.  a secluded residence, usually for religious sects"@en ;
      rdfs:subClassOf ontologyofspatialobject:Spot .

ontologyofspatialobject:metro-station
      a       owl:Class ;
      rdfs:comment "metro station.  metro station (Underground, Tube, or Metro)"@en ;
      rdfs:subClassOf ontologyofspatialobject:Spot .

ontologyofspatialobject:deep
      a       owl:Class ;
      rdfs:comment "deep.  a localized deep area within the confines of a larger feature, such as a trough, basin or trench"@en ;
      rdfs:subClassOf ontologyofspatialobject:Undersea .

ontologyofspatialobject:medical-center
      a       owl:Class ;
      rdfs:comment "medical center.  a complex of health care buildings including two or more of the following: hospital, medical school, clinic, pharmacy, doctor's offices, etc."@en ;
      rdfs:subClassOf ontologyofspatialobject:Spot .

ontologyofspatialobject:factory
      a       owl:Class ;
      rdfs:comment "factory.  one or more buildings where goods are manufactured, processed or fabricated"@en ;
      rdfs:subClassOf ontologyofspatialobject:Spot .

ontologyofspatialobject:canyon
      a       owl:Class ;
      rdfs:comment "canyon.  a relatively narrow, deep depression with steep sides, the bottom of which generally has a continuous slope"@en , "canyon.  a deep, narrow valley with steep sides cutting into a plateau or mountainous area"@en ;
      rdfs:subClassOf ontologyofspatialobject:Hypsographic , ontologyofspatialobject:Undersea .

ontologyofspatialobject:forest-station
      a       owl:Class ;
      rdfs:comment "forest station.  a collection of buildings and facilities for carrying out forest management"@en ;
      rdfs:subClassOf ontologyofspatialobject:Spot .

ontologyofspatialobject:population
      a       owl:FunctionalProperty , owl:DatatypeProperty ;
      rdfs:comment """the population (optional may be null).

Es utilizada por Geonames y por Wikipedia"""@en ;
      rdfs:domain ontologyofspatialobject:SpatialObject ;
      rdfs:range xsd:long ;
      rdfs:subPropertyOf owl:topDataProperty .

ontologyofspatialobject:traffic-circle
      a       owl:Class ;
      rdfs:comment "traffic circle.  a road junction formed around a central circle about which traffic moves in one direction only"@en ;
      rdfs:subClassOf ontologyofspatialobject:Spot .

ontologyofspatialobject:moraine
      a       owl:Class ;
      rdfs:comment "moraine.  a mound, ridge, or other accumulation of glacial till"@en ;
      rdfs:subClassOf ontologyofspatialobject:Hypsographic .

ontologyofspatialobject:State-Exam-Prep-Centre
      a       owl:Class ;
      rdfs:comment "State Exam Prep Centre.  state exam preparation centres"@en ;
      rdfs:subClassOf ontologyofspatialobject:Spot .

ontologyofspatialobject:fjords
      a       owl:Class ;
      rdfs:comment "fjords.  long, narrow, steep-walled, deep-water arms of the sea at high latitudes, usually along mountainous coasts"@en ;
      rdfs:subClassOf ontologyofspatialobject:Hydrographic .

ontologyofspatialobject:radio-observatory
      a       owl:Class ;
      rdfs:comment "radio observatory.  a facility equipped with an array of antennae for receiving radio waves from space"@en ;
      rdfs:subClassOf ontologyofspatialobject:Spot .

ontologyofspatialobject:sea
      a       owl:Class ;
      rdfs:comment "sea.  a large body of salt water more or less confined by continuous land or chains of islands forming a subdivision of an ocean"@en ;
      rdfs:subClassOf ontologyofspatialobject:Hydrographic .

ontologyofspatialobject:icecap-dome
      a       owl:Class ;
      rdfs:comment "icecap dome.  a comparatively elevated area on an icecap"@en ;
      rdfs:subClassOf ontologyofspatialobject:Hydrographic .

ontologyofspatialobject:abandoned-canal
      a       owl:Class ;
      rdfs:comment "abandoned canal.  "@en ;
      rdfs:subClassOf ontologyofspatialobject:Hydrographic .

ontologyofspatialobject:opera-house
      a       owl:Class ;
      rdfs:comment "opera house.  A theater designed chiefly for the performance of operas."@en ;
      rdfs:subClassOf ontologyofspatialobject:Spot .

<http://www.semanticweb.org/mpuebla/ontologies/2015/8/OntologyOfSpatialObject>
      a       owl:Ontology ;
      terms:license "http://creativecommons.org/licenses/by/3.0/" ;
      ontologyofspatialobject:creators
              "Copyright  2016 Manuel Puebla" ;
      owl:description "Descripcion."@en ;
      owl:preferredNamespacePrefix
              "OntologyofSpatiaObject" ;
      owl:preferredNamespaceUri
              "http://purl.org/vocommons/voaf#OntologyofSpatiaObject#" ;
      owl:title "Titulo"@en .

ontologyofspatialobject:coalfield
      a       owl:Class ;
      rdfs:comment "coalfield.  a region in which coal deposits of possible economic value occur"@en ;
      rdfs:subClassOf ontologyofspatialobject:Area .

[]    a       owl:AllDisjointProperties ;
      owl:members (ontologyofspatialobject:adminName4 ontologyofspatialobject:elevation ontologyofspatialobject:language ontologyofspatialobject:timezone ontologyofspatialobject:title ontologyofspatialobject:typeRelation ontologyofspatialobject:wikipediaUrl ontologyofspatialobject:wkt) .

ontologyofspatialobject:mereological
      a       owl:TransitiveProperty , owl:ObjectProperty , owl:SymmetricProperty ;
      rdfs:comment """Mereological relations

En filosofia, la mereologia es el estudio de las relaciones entre partes, tanto de las partes con el todo, como de las partes con otras partes.

Tengo dudas en la relacion que existe entre las relaciones \"Mereological\"  con \"inside\" y \"contains\". Parecen ser equivalentes \"isPartOf\" con \"inside\"  y  \"isWholeOf\"  con \"contains\" en http://kauppinen.net/tomi/kauppinen-xmlfinland2009.pdf hay ejemplos de relaciones Mereological. 

No estoy seguro, pero la diferencia que noto es que las Mereological no estan implicadas necesariamente por su ubicacion espacial sino por su estructura organizacional. Pero por que las ubican como relaciones espaciales en la literatura.
Ejemplo tabla empresas y tabla trabajadores. Imaginen que los trabajadores estan ubicados espacialmente. Un trabajador es parte de un empresa y la empresa tiene parte (has-part o isWholeOf) de ese trabador, pero el trabajador no hay una relacion de ubicacion espacial entre el trabajador y la empresa(relaciones \"inside\" y \"contains\")"""@en ;
      rdfs:domain ontologyofspatialobject:SpatialObject ;
      rdfs:range ontologyofspatialobject:SpatialObject ;
      rdfs:subPropertyOf ontologyofspatialobject:spatial .

ontologyofspatialobject:tablemounts--or-guyots-
      a       owl:Class ;
      rdfs:comment "tablemounts (or guyots).  seamounts having a comparatively smooth, flat top"@en ;
      rdfs:subClassOf ontologyofspatialobject:Undersea .

ontologyofspatialobject:agricultural-school
      a       owl:Class ;
      rdfs:comment "agricultural school.  a school with a curriculum focused on agriculture"@en ;
      rdfs:subClassOf ontologyofspatialobject:Spot .

ontologyofspatialobject:hut
      a       owl:Class ;
      rdfs:comment "hut.  a small primitive house"@en ;
      rdfs:subClassOf ontologyofspatialobject:Spot .

ontologyofspatialobject:section-of-plateau
      a       owl:Class ;
      rdfs:comment "section of plateau.  "@en ;
      rdfs:subClassOf ontologyofspatialobject:Hypsographic .

ontologyofspatialobject:pyramids
      a       owl:Class ;
      rdfs:comment "pyramids.  ancient massive structures of square ground plan with four triangular faces meeting at a point and used for enclosing tombs"@en ;
      rdfs:subClassOf ontologyofspatialobject:Spot .

ontologyofspatialobject:technical-school
      a       owl:Class ;
      rdfs:comment "technical school.  post-secondary school with a specifically technical or vocational curriculum"@en ;
      rdfs:subClassOf ontologyofspatialobject:Spot .

ontologyofspatialobject:hill
      a       owl:Class ;
      rdfs:comment "hill.  a rounded elevation of limited extent rising above the surrounding land with local relief of less than 300m"@en , "hill.  an elevation rising generally less than 500 meters"@en ;
      rdfs:subClassOf ontologyofspatialobject:Hypsographic , ontologyofspatialobject:Undersea .

ontologyofspatialobject:section-of-estate
      a       owl:Class ;
      rdfs:comment "section of estate.  "@en ;
      rdfs:subClassOf ontologyofspatialobject:Spot .

ontologyofspatialobject:featureClass
      a       owl:FunctionalProperty , owl:DatatypeProperty ;
      rdfs:comment "character A,H,L,P,R,S,T,U,V"@en ;
      rdfs:domain ontologyofspatialobject:SpatialObject ;
      rdfs:range xsd:string ;
      rdfs:subPropertyOf ontologyofspatialobject:gonameDataProperty .

ontologyofspatialobject:oil-pipeline-junction
      a       owl:Class ;
      rdfs:comment "oil pipeline junction.  a section of an oil pipeline where two or more pipes join together"@en ;
      rdfs:subClassOf ontologyofspatialobject:Spot .

ontologyofspatialobject:anchorage
      a       owl:Class ;
      rdfs:comment "anchorage.  an area where vessels may anchor"@en ;
      rdfs:subClassOf ontologyofspatialobject:Hydrographic .

ontologyofspatialobject:section-of-waterfall-s-
      a       owl:Class ;
      rdfs:comment "section of waterfall(s).  "@en ;
      rdfs:subClassOf ontologyofspatialobject:Hydrographic .

ontologyofspatialobject:shelf-valley
      a       owl:Class ;
      rdfs:comment "shelf valley.  a valley on the shelf, generally the shoreward extension of a canyon"@en ;
      rdfs:subClassOf ontologyofspatialobject:Undersea .

ontologyofspatialobject:shelf-edge
      a       owl:Class ;
      rdfs:comment "shelf edge.  a line along which there is a marked increase of slope at the outer margin of a continental shelf or island shelf"@en ;
      rdfs:subClassOf ontologyofspatialobject:Undersea .

ontologyofspatialobject:abandoned-mission
      a       owl:Class ;
      rdfs:comment "abandoned mission.  "@en ;
      rdfs:subClassOf ontologyofspatialobject:Spot .

ontologyofspatialobject:facility-center
      a       owl:Class ;
      rdfs:comment "facility center.  a place where more than one facility is situated"@en ;
      rdfs:subClassOf ontologyofspatialobject:Spot .

ontologyofspatialobject:pans
      a       owl:Class ;
      rdfs:comment "pans.  a near-level shallow, natural depression or basin, usually containing an intermittent lake, pond, or pool"@en ;
      rdfs:subClassOf ontologyofspatialobject:Hypsographic .

ontologyofspatialobject:icecap-depression
      a       owl:Class ;
      rdfs:comment "icecap depression.  a comparatively depressed area on an icecap"@en ;
      rdfs:subClassOf ontologyofspatialobject:Hydrographic .

ontologyofspatialobject:featureCode
      a       owl:FunctionalProperty , owl:DatatypeProperty ;
      rdfs:comment "featureCode"@en ;
      rdfs:domain ontologyofspatialobject:SpatialObject ;
      rdfs:range xsd:string ;
      rdfs:subPropertyOf ontologyofspatialobject:gonameDataProperty .

ontologyofspatialobject:school
      a       owl:Class ;
      rdfs:comment "school.  building(s) where instruction in one or more branches of knowledge takes place"@en ;
      rdfs:subClassOf ontologyofspatialobject:Spot .

ontologyofspatialobject:naval-base
      a       owl:Class ;
      rdfs:comment "naval base.  an area used to store supplies, provide barracks for troops and naval personnel, a port for naval vessels, and from which operations are initiated"@en ;
      rdfs:subClassOf ontologyofspatialobject:Area .

ontologyofspatialobject:meteorological-station
      a       owl:Class ;
      rdfs:comment "meteorological station.  a station at which weather elements are recorded"@en ;
      rdfs:subClassOf ontologyofspatialobject:Spot .

ontologyofspatialobject:burial-cave-s-
      a       owl:Class ;
      rdfs:comment "burial cave(s).  a cave used for human burials"@en ;
      rdfs:subClassOf ontologyofspatialobject:Spot .

ontologyofspatialobject:diplomatic-facility
      a       owl:Class ;
      rdfs:comment "diplomatic facility.  office, residence, or facility of a foreign government, which may include an embassy, consulate, chancery, office of charge d'affaires, or other diplomatic, economic, military, or cultural mission"@en ;
      rdfs:subClassOf ontologyofspatialobject:Spot .

ontologyofspatialobject:dependent-political-entity
      a       owl:Class ;
      rdfs:comment "dependent political entity.  "@en ;
      rdfs:subClassOf ontologyofspatialobject:AdministrativeBoundary .

ontologyofspatialobject:ancient-site
      a       owl:Class ;
      rdfs:comment "ancient site.  a place where archeological remains, old structures, or cultural artifacts are located"@en ;
      rdfs:subClassOf ontologyofspatialobject:Spot .

ontologyofspatialobject:populated-places
      a       owl:Class ;
      rdfs:comment "populated places.  cities, towns, villages, or other agglomerations of buildings where people live and work"@en ;
      rdfs:subClassOf ontologyofspatialobject:PopulatedPlace .
